Refactoring - global assumptions, locales

Properties.thy
@@ -1,19 +1,16 @@
 theory Properties
-  imports Reachability
+  imports Reachability MoreList
 begin
 
-context ProofVerifier
+context StrongHashProofVerifier
 begin
 
 
 (* ------------------------------------------------------------------------------------ *)
-
 text \<open>There are no double deposits\<close>
 theorem callDepositNoDouble:
   assumes "callDeposit contracts address block msg ID token amount = (Success, contracts')"         
   assumes "reachableFrom contracts' contracts'' steps"
-  (* NOTE: additional assumption *)
-  assumes "hash3 (sender msg) token amount \<noteq> 0"
   shows "fst (callDeposit contracts'' address block' msg' ID token' amount') \<noteq> Success"
 proof (cases "bridgeDead contracts'' address")
   case False
@@ -21,7 +18,7 @@ proof (cases "bridgeDead contracts'' address")
     using callDepositWritesHash[OF assms(1)]
     by simp
   then have "getDeposit (the (tokenDepositState contracts'' address)) ID \<noteq> 0"
-    using False reachableFromGetDepositBridgeNotDead assms
+    using False reachableFromGetDepositBridgeNotDead hash3_nonzero[of "sender msg" token amount] assms
     by auto
   then show ?thesis
     using callDepositWrittenHash by blast
@@ -31,6 +28,11 @@ next
     using callDepositFailsInDeadState 
     by presburger
 qed
+
+end
+
+context HashProofVerifier
+begin
 
 text \<open>There are no double claims\<close>
 theorem callClaimNoDouble:
@@ -54,12 +56,15 @@ proof-
     by (auto simp add: Let_def split: option.splits prod.splits)
 qed
 
+end
+
+context StrongHashProofVerifier
+begin
+
 text \<open>There are no double cancels\<close>
 theorem callCancelNoDouble:
   assumes "callCancelDepositWhileDead contracts address msg block ID token amount proof = (Success, contracts')"
   assumes "reachableFrom contracts' contracts'' steps"
-  (* NOTE: additional assumption *)
-  assumes "hash3 (sender msg') token' amount' \<noteq> 0"
   shows "fst (callCancelDepositWhileDead contracts'' address msg' block' ID token' amount' proof') \<noteq> Success"
 proof-
   have "getDeposit (the (tokenDepositState contracts' address)) ID = 0"
@@ -77,6 +82,11 @@ proof-
     by (metis fstI surj_pair)
 qed
 
+end
+
+context HashProofVerifier
+begin
+
 lemma callWithdrawWhileDeadNoDouble:
   assumes "callWithdrawWhileDead contracts address msg block token amount proof = (Success, contracts')"
   assumes "reachableFrom contracts' contracts'' steps"
@@ -93,13 +103,17 @@ proof-
     by (metis prod.collapse)
 qed
 
+end
+
 (* ------------------------------------------------------------------------------------ *)
+
+context StrongHashProofVerifier
+begin
 
 text \<open>We want to prove that there cannot be two DEPOSIT steps with the same ID on the same tokenDeposit address\<close>
 
 lemma DEPOSITNoDoubleCons:
   assumes "reachableFrom contracts contracts' (DEPOSIT tokenDepositAddress caller ID token amount # steps)"
-  assumes "\<forall> step \<in> set steps. \<forall> caller' amount' ID' token'. step = DEPOSIT tokenDepositAddress caller' ID' token' amount' \<longrightarrow> hash3 caller' token' amount' \<noteq> 0"
   shows "\<nexists> token' caller' amount'. DEPOSIT tokenDepositAddress caller' ID token' amount' \<in> set steps"
 proof (rule ccontr)
   obtain contracts'' block where *:
@@ -110,7 +124,7 @@ proof (rule ccontr)
 
   moreover
 
-  assume "~ ?thesis"
+  assume "\<not> ?thesis"
   then obtain token' caller' amount' where **: "DEPOSIT tokenDepositAddress caller' ID token' amount' \<in> set steps"
     by auto
   obtain c1 c2 steps1 steps2 block' where ***:
@@ -127,9 +141,6 @@ proof (rule ccontr)
   next
     show "reachableFrom c2 contracts'' steps1"
       by fact
-  next
-    show "hash3 (sender (message caller' amount')) token' amount' \<noteq> 0"
-      using "**" assms message_def by force
   qed
 
   ultimately
@@ -141,7 +152,6 @@ qed
 lemma DEPOSITNoDouble:
   assumes "reachableFrom contracts contracts' steps"
   assumes "steps = steps1 @ [DEPOSIT tokenDepositAddress caller ID token amount] @ steps2 @ [DEPOSIT tokenDepositAddress caller' ID token' amount'] @ steps3"
-  assumes "\<forall> step \<in> set steps. \<forall> caller' amount' ID' token'. step = DEPOSIT tokenDepositAddress caller' ID' token' amount' \<longrightarrow> hash3 caller' token' amount' \<noteq> 0"
   shows False
 proof-
   obtain contracts'' where *: 
@@ -152,7 +162,7 @@ proof-
  
   have "\<nexists> token'' caller'' amount''. DEPOSIT tokenDepositAddress caller'' ID token'' amount'' \<in> set (steps2 @ [DEPOSIT tokenDepositAddress caller' ID token' amount'] @ steps3)"
     using DEPOSITNoDoubleCons[OF *(2)] assms
-    by (metis Un_iff set_append)
+    by metis
   then show False
     by auto
 qed
@@ -160,7 +170,6 @@ qed
 lemma DEPOSITNoDouble':
   assumes "reachableFrom contracts contracts' steps"
   assumes "steps = steps1 @ [DEPOSIT tokenDepositAddress caller ID token amount] @ steps2"
-  assumes "\<forall> step \<in> set steps. \<forall> caller' amount' ID' token'. step = DEPOSIT tokenDepositAddress caller' ID' token' amount' \<longrightarrow> hash3 caller' token' amount' \<noteq> 0"
   shows "\<nexists> token' caller' amount'. DEPOSIT tokenDepositAddress caller' ID token' amount' \<in> set (steps1 @ steps2)"
 proof (rule ccontr)
   assume "\<not> ?thesis"
@@ -185,6 +194,11 @@ proof (rule ccontr)
       by auto
   qed
 qed
+
+end
+
+context HashProofVerifier
+begin
 
 text \<open>We want to prove that there cannot be two CLAIM steps with the same ID on the same bridge address\<close>
 
@@ -262,353 +276,299 @@ proof (rule ccontr)
   qed
 qed
 
+end
+
 (* ------------------------------------------------------------------------------------ *)
 
-text \<open>No deposit after the bridge dies\<close>
-theorem  noDepositBridgeDead: 
-  assumes "bridgeDead contracts tokenDepositAddress"
-  assumes "reachableFrom contracts contracts' steps"
-  shows "fst (callDeposit contracts' tokenDepositAddress block msg ID token amount) \<noteq> Success"
-  using assms callDepositFailsInDeadState reachableFromDeadState
+(*
+                         update                    [stepsNoUpdate]             
+   contractsLastUpdate'    \<rightarrow>   contractsLastUpdate      \<rightarrow>*    contractsLU
+   properSetup                      noUpdates                  
+*)
+locale LastUpdate = StrongHashProofVerifier + 
+  fixes contractsLastUpdate' :: Contracts
+  fixes contractsLastUpdate :: Contracts
+  fixes contractsLU :: Contracts
+  fixes stepsNoUpdate :: "Step list"
+  fixes blockLU :: Block
+  fixes blockNumLU :: uint256
+  fixes stateRoot :: bytes32
+  fixes tokenDepositAddress :: address
+  fixes bridgeAddress :: address
+
+  \<comment> \<open>starting from a properly configured state\<close>
+  assumes properSetupLastUpdate':
+   "properSetup contractsLastUpdate' tokenDepositAddress bridgeAddress"
+  \<comment> \<open>the last update that happened\<close>
+  assumes lastUpdate:
+    "let stateOracleAddress = stateOracleAddressB contractsLastUpdate' bridgeAddress
+      in callUpdate contractsLastUpdate' stateOracleAddress blockLU blockNumLU stateRoot = (Success, contractsLastUpdate)"
+  \<comment> \<open>there were no updates since then\<close>
+  assumes reachableFromLastUpdateLU: 
+    "reachableFrom contractsLastUpdate contractsLU stepsNoUpdate"
+  assumes noUpdate:
+    "let stateOracleAddress = stateOracleAddressB contractsLastUpdate bridgeAddress
+      in \<nexists> stateRoot'. UPDATE stateOracleAddress stateRoot' \<in> set stepsNoUpdate"
+begin
+
+definition UPDATE_step where
+  "UPDATE_step = UPDATE (stateOracleAddressB contractsLastUpdate' bridgeAddress) stateRoot"
+
+lemma reachableFromLastUpdate'LastUpdate [simp]:
+  shows "reachableFrom contractsLastUpdate' contractsLastUpdate [UPDATE_step]"
+proof-
+  have "executeStep contractsLastUpdate' blockNumLU blockLU (UPDATE_step) = (Success, contractsLastUpdate)"
+    using lastUpdate
+    unfolding UPDATE_step_def
+    by simp
+  then show ?thesis
+    using reachableFrom_base reachableFrom_step by blast
+qed
+
+lemma reachableFromLastUpdate'LU [simp]:
+  shows "reachableFrom contractsLastUpdate' contractsLU (stepsNoUpdate @ [UPDATE_step])"
+  using reachableFromTrans[OF reachableFromLastUpdateLU reachableFromLastUpdate'LastUpdate]
+  by simp
+
+lemma properSetupLastUpdate [simp]:
+  shows "properSetup contractsLastUpdate tokenDepositAddress bridgeAddress"
+  using callUpdateProperSetup lastUpdate properSetupLastUpdate' 
+  by presburger
+
+lemma properSetupLU [simp]:
+  shows "properSetup contractsLU tokenDepositAddress bridgeAddress"
+  using reachableFromLastUpdateLU 
+  by auto
+
+lemma stateOracleAddressBLU [simp]:
+  shows "stateOracleAddressB contractsLU bridgeAddress =
+         stateOracleAddressB contractsLastUpdate' bridgeAddress"
+  using reachableFromBridgeStateOracle reachableFromLastUpdate'LU 
   by blast
 
+lemma depositLastUpdate' [simp]: 
+  shows "BridgeState.deposit (the (bridgeState contractsLastUpdate' bridgeAddress)) = tokenDepositAddress"
+  by (meson properSetupLastUpdate' properSetup_def)
 
-text \<open>After a successful deposit and a state update, 
-      if a bridge is still alive a claim can be made \<close>
-theorem claimPossibleAfterDepositAndUpdate:
-  \<comment> \<open>contracts are setup properly in the initial state, for the given token\<close>
-  assumes "properSetup contracts tokenDepositAddress bridgeAddress"
-  assumes "properToken contracts tokenDepositAddress bridgeAddress token"
+lemma depositLU [simp]:
+  "BridgeState.deposit (the (bridgeState contractsLU bridgeAddress)) = tokenDepositAddress"
+  using reachableFromBridgeDeposit reachableFromLastUpdate'LU depositLastUpdate'
+  by blast
 
-  \<comment> \<open>A deposit is successfully made\<close>
-  assumes "callDeposit contracts tokenDepositAddress block msg ID token amount = (Success, contractsD)"
-  \<comment> \<open>after a deposit a new state is reached\<close>
-  assumes "reachableFrom contractsD contractsD' steps"
-  \<comment> \<open>the bridge is not dead in the reached state\<close>
-  assumes "\<not> bridgeDead  contractsD' tokenDepositAddress"
-  \<comment> \<open>A last update is made\<close>
-  assumes "let stateOracleAddress = stateOracleAddressTD contractsD' tokenDepositAddress
-            in callUpdate contractsD' stateOracleAddress block blockNum stateRoot = (Success, contractsU)"
-  \<comment> \<open>A new state is reached after that last update\<close>
-  assumes "reachableFrom contractsU contractsU' steps'"
-  assumes noUpdates:
-          "let stateOracleAddress = stateOracleAddressTD contractsU tokenDepositAddress
-            in \<nexists> stateRoot'. UPDATE stateOracleAddress stateRoot' \<in> set steps'"
+lemma tokenDepositStateLastUpdate'NotNone [simp]:
+  shows "tokenDepositState contractsLastUpdate' tokenDepositAddress \<noteq> None"
+  by (meson properSetupLastUpdate' properSetup_def)
 
-  \<comment> \<open>there was no previous claim\<close>
-  assumes "getClaim (the (bridgeState contractsU' bridgeAddress)) ID = False"
+lemma callLastStateLU [simp]:
+  shows "callLastState contractsLU (stateOracleAddressB contractsLU bridgeAddress) = 
+         (Success, stateRoot)"
+  using noUpdate noUpdateLastState callUpdateLastState lastUpdate
+  using reachableFromBridgeStateOracle reachableFromLastUpdate'LU reachableFromLastUpdateLU
+  by (smt (verit, ccfv_threshold) callLastState_def  option.case_eq_if properSetupLU properSetup_def )
 
-  \<comment> \<open>The same person who made the deposit can make the claim\<close>
-  assumes "sender msg' = sender msg"
+lemma getLastStateBLU [simp]:
+  shows "getLastStateB contractsLU bridgeAddress = stateRoot"
+  using callLastState callLastStateLU
+  by blast
 
-  assumes "hash3 (sender msg) token amount \<noteq> 0" (* Additional assumption *)
+lemma  getLastStateTDLU [simp]:
+  shows "getLastStateTD contractsLU tokenDepositAddress = stateRoot"
+  by (metis getLastStateBLU properSetupLU properSetup_getLastState)
 
-  \<comment> \<open>A claim can be made with the state root and the proof obtained from the state that
-      was used for the last update\<close>
-  shows "let stateRoot = generateStateRoot contractsD';
-             proof = generateDepositProof contractsD' ID
-          in \<exists> contractsC. callClaim contractsU' bridgeAddress msg' ID token amount proof = (Success, contractsC)"
-proof-
-  define stateOracleAddress where 
-       "stateOracleAddress = BridgeState.stateOracle (the (bridgeState contracts bridgeAddress))"
-  define proofVerifierAddress where 
-       "proofVerifierAddress = BridgeState.proofVerifier (the (bridgeState contracts bridgeAddress))"
-  define tokenPairsAddress where 
-       "tokenPairsAddress = BridgeState.tokenPairs (the (bridgeState contracts bridgeAddress))"
-  define "proof" where "proof = generateDepositProof contractsD' ID"
-  define stateRoot where "stateRoot = generateStateRoot contractsD'"
+lemma generateStateRootLastUpdate' [simp]:
+  shows "generateStateRoot contractsLastUpdate' = stateRoot"
+  using lastUpdate updateSuccess 
+  by force
 
-  have "verifyDepositProof () tokenDepositAddress ID (hash3 (sender msg) token amount) stateRoot proof = True"
-  proof (rule verifyDepositProofI)
-    show "generateDepositProof contractsD' ID = proof"
-      unfolding proof_def
-      by simp
-  next
-    show "generateStateRoot contractsD' = stateRoot"
-      unfolding stateRoot_def
-      by simp
-  next
-    have "tokenDepositState contractsD tokenDepositAddress \<noteq> None"
-      using \<open>callDeposit contracts tokenDepositAddress block msg ID token amount = (Success, contractsD)\<close>
-      using callDepositE by blast
-    then have "tokenDepositState contractsD' tokenDepositAddress \<noteq> None"
-      using \<open>reachableFrom contractsD contractsD' steps\<close>
-      using reachableFromTokenDepositState by blast
-    then show "tokenDepositState contractsD' tokenDepositAddress = Some (the (tokenDepositState contractsD' tokenDepositAddress))"
-      by simp
-  next
-    show "getDeposit (the (tokenDepositState contractsD' tokenDepositAddress)) ID = hash3 (sender msg) token amount"
-    proof (rule reachableFromGetDepositBridgeNotDead)
-      show "reachableFrom contractsD contractsD' steps" 
-        by fact
-    next
-      show "hash3 (sender msg) token amount \<noteq> 0"
-        by fact
-    next
-      show "getDeposit (the (tokenDepositState contractsD tokenDepositAddress)) ID = hash3 (sender msg) token amount"
-        using callDepositWritesHash assms
-        by blast
-    next
-      show "\<not> bridgeDead contractsD' tokenDepositAddress"
-        using assms
-        by simp
-    qed
-  qed
-
-  have "bridgeState contractsU bridgeAddress \<noteq> None"
-    using reachableFromBridgeState assms
-    unfolding properSetup_def
-    by (auto simp add: Let_def)
-  then have "bridgeState contractsU' bridgeAddress \<noteq> None"
-    using \<open>reachableFrom contractsU contractsU' steps'\<close> reachableFromBridgeState
-    by blast
-  then obtain stateBridgeU' where 
-    "bridgeState contractsU' bridgeAddress = Some stateBridgeU'"
-    by auto
-  then have stateBridgeU: "stateBridgeU' = the (bridgeState contractsU' bridgeAddress)"
-    using \<open>bridgeState contractsU bridgeAddress \<noteq> None\<close>
-    by auto
-
-  have "stateOracleAddressTD contractsU tokenDepositAddress = stateOracleAddress"
-    using assms stateOracleAddress_def properSetup_def
-    by (auto simp add: Let_def)
-  then have "stateOracleAddressTD contractsU' tokenDepositAddress = stateOracleAddress"
-    using \<open>reachableFrom contractsU contractsU' steps'\<close> reachableFromDepositStateOracle by blast
-
-  have "BridgeState.stateOracle stateBridgeU' = stateOracleAddress"
-       "BridgeState.proofVerifier stateBridgeU' = proofVerifierAddress"
-       "BridgeState.deposit stateBridgeU' = tokenDepositAddress"
-       "tokenPairsState contractsU' (BridgeState.tokenPairs stateBridgeU') \<noteq> None"
-    using assms stateBridgeU \<open>bridgeState contractsU bridgeAddress \<noteq> None\<close> properSetup_def stateOracleAddress_def proofVerifierAddress_def
-    by (auto simp add: Let_def)
-
-  then obtain stateTokenPairs where
-    stateTokenPairs: "tokenPairsState contractsU' (BridgeState.tokenPairs stateBridgeU') = Some stateTokenPairs"
-    by auto
-
-  have "StateOracleState.lastState (the (stateOracleState contractsU stateOracleAddress)) = stateRoot"
-    using assms \<open>stateOracleAddressTD contractsU tokenDepositAddress = stateOracleAddress\<close>
-    unfolding stateRoot_def
-    by (simp add: updateSuccess)
-  then have "StateOracleState.lastState (the (stateOracleState contractsU' stateOracleAddress)) = stateRoot"
-    using \<open>reachableFrom contractsU contractsU' steps'\<close> noUpdates
-    using  \<open>stateOracleAddressTD contractsU tokenDepositAddress = stateOracleAddress\<close> 
-    by (metis  noUpdateLastState)
-
-  have "fst (callClaim contractsU' bridgeAddress msg' ID token amount proof) = Success"
-  proof (rule callClaimI)
-    show "bridgeState contractsU' bridgeAddress = Some stateBridgeU'"
-      by fact
-  next
-    show "verifyDepositProof () (BridgeState.deposit stateBridgeU') ID (hash3 (sender msg') token amount)  
-          (StateOracleState.lastState (the (stateOracleState contractsU' (BridgeState.stateOracle stateBridgeU')))) proof"
-      using \<open>BridgeState.deposit stateBridgeU' = tokenDepositAddress\<close>
-      using \<open>bridgeState contractsU' bridgeAddress = Some stateBridgeU'\<close>
-      using \<open>BridgeState.stateOracle stateBridgeU' = stateOracleAddress\<close>
-      using \<open>StateOracleState.lastState (the (stateOracleState contractsU' stateOracleAddress)) = stateRoot\<close>
-      using \<open>verifyDepositProof () tokenDepositAddress ID (hash3 (sender msg) token amount) stateRoot proof = True\<close>
-      using \<open>sender msg' = sender msg\<close>
-      by simp
-  next
-    show "tokenPairsState contractsU' (BridgeState.tokenPairs stateBridgeU') = Some stateTokenPairs"
-      using \<open>bridgeState contractsU' bridgeAddress = Some stateBridgeU'\<close>
-            \<open>tokenPairsState contractsU' (BridgeState.tokenPairs stateBridgeU') = Some stateTokenPairs\<close> 
-      by auto
-  next
-    show "stateOracleState contractsU' (BridgeState.stateOracle stateBridgeU') =
-          Some (the (stateOracleState contractsU' (BridgeState.stateOracle stateBridgeU')))"
-      using assms
-      by (metis callDepositProperSetup callUpdateProperSetup option.collapse properSetupReachable properSetup_def stateBridgeU)
-  next
-    show "proofVerifierState contractsU' (BridgeState.proofVerifier stateBridgeU') \<noteq> None"
-      using \<open>BridgeState.proofVerifier stateBridgeU' = proofVerifierAddress\<close> 
-            stateBridgeU 
-      using assms
-      using callDepositIProofVerifier callUpdateIProofVerifier reachableFromIProofVerifier
-      unfolding proofVerifierAddress_def properSetup_def
-      by metis
-  next
-    show "getMinted stateTokenPairs token \<noteq> 0"
-      using stateTokenPairs assms stateBridgeU
-      unfolding properToken_def
-      by (auto simp add: Let_def)
-  next
-    show "ERC20state contractsU' (getMinted stateTokenPairs token) \<noteq> None"
-      using assms
-      unfolding properToken_def
-      by (smt (verit, ccfv_SIG) assms(2) callDepositProperToken callUpdateIBridge callUpdateIERC20 callUpdateITokenPairs option.sel properToken_def reachableFromBridgeTokenPairs reachableFromERC20State reachableFromITokenPairs stateBridgeU stateTokenPairs)
-  next
-    show "getClaim stateBridgeU' ID = False"
-      using \<open>bridgeState contractsU' bridgeAddress = Some stateBridgeU'\<close> assms 
-      by auto
-  qed
-  then show ?thesis 
-    unfolding Let_def proof_def
-    by (metis eq_fst_iff)
-qed
-
-(* ------------------------------------------------------------------------------------ *)
-
-text \<open>If claim succeeds, then there must be a previous deposit transaction hash written in the deposits array\<close>
-lemma callClaimGetDeposit:
-  \<comment> \<open>starting from a properly configured state\<close>
-  assumes "properSetup contracts tokenDepositAddress bridgeAddress"
-  \<comment> \<open>the last update that happened\<close>
-  assumes update:
-          "let stateOracleAddress = stateOracleAddressB contracts bridgeAddress
-            in callUpdate contracts stateOracleAddress block blockNum stateRoot = (Success, contracts')"
-  \<comment> \<open>there were no updates since then\<close>
-  assumes "reachableFrom contracts' contracts'' steps'"
-  assumes noUpdate:
-          "let stateOracleAddress = stateOracleAddressB contracts bridgeAddress
-            in \<nexists> stateRoot'. UPDATE stateOracleAddress stateRoot' \<in> set steps'"
-
+theorem callClaimGetDeposit:
   \<comment> \<open>claim succeded\<close>
-  assumes claim: "callClaim contracts'' bridgeAddress msg ID token amount proof = (Success, contracts''')"
-
-  shows "getDeposit (the (tokenDepositState contracts' tokenDepositAddress)) ID = hash3 (sender msg) token amount"
+  assumes claim: "callClaim contractsLU bridgeAddress msg ID token amount proof = (Success, contractsClaim)"
+  shows "getDeposit (the (tokenDepositState contractsLastUpdate' tokenDepositAddress)) ID = hash3 (sender msg) token amount"
 proof-
-  define stateBridge where "stateBridge = the (bridgeState contracts'' bridgeAddress)"
-  define stateStateOracle where "stateStateOracle = the (stateOracleState contracts'' (BridgeState.stateOracle stateBridge))"
-  define stateTokenDeposit where "stateTokenDeposit = the (tokenDepositState contracts'' tokenDepositAddress)"
-
-  have dB: "BridgeState.deposit stateBridge = tokenDepositAddress"
-    using assms
-    unfolding stateBridge_def properSetup_def Let_def
-    by auto
-
-  have sOB: "BridgeState.stateOracle stateBridge = stateOracleAddressB contracts bridgeAddress"
-    using assms
-    unfolding stateBridge_def
-    by simp
-
-  have "properSetup contracts' tokenDepositAddress bridgeAddress"
-    using assms
-    by (meson callUpdateProperSetup properSetupReachable)
-
-  obtain stateRoot where stateLast: "callLastState contracts'' (BridgeState.stateOracle stateBridge) = (Success, stateRoot)"
-    using claim
-    by (metis callClaimCallLastState stateBridge_def)
-  then have 1: "StateOracleState.lastState stateStateOracle = stateRoot"
-    unfolding stateStateOracle_def
-    using callLastState 
-    by blast
-  then have "getLastStateB contracts'' bridgeAddress = stateRoot"
-    using stateBridge_def stateStateOracle_def by blast
-  then have "getLastStateB contracts' bridgeAddress = stateRoot"
-    using \<open>reachableFrom contracts' contracts'' steps'\<close> noUpdate
-    using reachableFromBridgeStateOracle
-    using noUpdateLastState sOB
-    by (metis stateBridge_def)
-
-  have "callVerifyDepositProof contracts'' (BridgeState.proofVerifier stateBridge) (BridgeState.deposit stateBridge) ID (hash3 (sender msg) token amount)
+  define stateBridge where "stateBridge = the (bridgeState contractsLU bridgeAddress)"
+  have "callVerifyDepositProof contractsLU (BridgeState.proofVerifier stateBridge) (BridgeState.deposit stateBridge) ID (hash3 (sender msg) token amount)
          stateRoot proof = Success"
-    using callClaimCallVerifyProof[OF claim] 1
-    unfolding stateBridge_def Let_def stateStateOracle_def
-    by blast
-  then have *: "verifyDepositProof () (BridgeState.deposit stateBridge) ID (hash3 (sender msg) token amount) stateRoot proof = True"
-    unfolding callVerifyDepositProof_def
+    using callClaimCallVerifyProof[OF claim] getLastStateBLU
+    unfolding stateBridge_def Let_def
+    by simp
+  then have "verifyDepositProof () tokenDepositAddress ID (hash3 (sender msg) token amount) stateRoot proof = True"
+    unfolding callVerifyDepositProof_def stateBridge_def
     by (simp split: option.splits if_split_asm)
-  show "getDeposit (the (tokenDepositState contracts' tokenDepositAddress)) ID =
-        hash3 (sender msg) token amount"
-  proof (rule verifyDepositProofE[OF _  *])
-    show "generateStateRoot contracts = stateRoot"
-      using updateSuccess update
-      using \<open>getLastStateB contracts' bridgeAddress = stateRoot\<close> by auto
-  next
-    show "tokenDepositState contracts (BridgeState.deposit stateBridge) =
-          Some (the (tokenDepositState contracts' tokenDepositAddress))"
-      using \<open>properSetup contracts' tokenDepositAddress bridgeAddress\<close> 
-      by (metis callUpdateITokenDeposit dB option.collapse properSetup_def update)
-  qed
+  then show ?thesis
+    using verifyDepositProofE
+    by (metis generateStateRootLastUpdate' option.collapse tokenDepositStateLastUpdate'NotNone)
 qed
+
+end
+
+locale Init' = StrongHashProofVerifier + 
+  fixes tokenDepositAddress :: address
+  fixes bridgeAddress :: address
+  fixes contractsInit :: Contracts
+  \<comment> \<open>The operation starts from an initial state that is properly setup\<close>
+  assumes properSetupInit [simp]:
+    "properSetup contractsInit tokenDepositAddress bridgeAddress"
+  \<comment> \<open>All relevant data is still empty\<close>
+  assumes depositsEmpty [simp]: 
+    "\<And> ID. getDeposit (the (tokenDepositState contractsInit tokenDepositAddress)) ID = 0"
+  assumes claimsEmpty [simp]:
+    "\<And> ID. getClaim (the (bridgeState contractsInit bridgeAddress)) ID = False"
+  assumes lastStateBZero [simp]:
+    "getLastStateB contractsInit bridgeAddress = 0"
+
+locale Init = Init' + 
+  fixes contractsI :: Contracts
+  fixes stepsInit :: "Step list"
+  assumes reachableFromInitI [simp]:
+    "reachableFrom contractsInit contractsI stepsInit"
+begin
+lemma lastStateTDZero [simp]:
+  shows "getLastStateTD contractsInit tokenDepositAddress = 0"
+  by (metis lastStateBZero properSetupInit properSetup_getLastState)
+end
+
+locale InitFirstUpdate = Init + 
+  fixes stateRootInit :: "bytes32"
+  assumes firstUpdate:
+    "stepsInit \<noteq> [] \<and> last stepsInit = UPDATE (stateOracleAddressB contractsInit bridgeAddress) stateRootInit"
+  assumes updatesNonZeroInit [simp]:
+    "updatesNonZero stepsInit"
+begin
+
+lemma stateRootInitNonZero:
+  "stateRootInit \<noteq> 0"
+  using firstUpdate updatesNonZeroInit
+  unfolding updatesNonZero_def
+  by (metis last_in_set)
+
+definition UPDATE1_step where 
+  "UPDATE1_step = UPDATE (stateOracleAddressB contractsInit bridgeAddress) stateRootInit"
+
+lemma obtainContractsU:
+  obtains blockU blockNumU contractsU where
+  "callUpdate contractsInit (stateOracleAddressB contractsInit bridgeAddress) blockU blockNumU stateRootInit = (Success, contractsU)" and
+  "reachableFrom contractsU contractsI (butlast stepsInit)"
+proof-
+  obtain steps where "stepsInit = steps @ [UPDATE1_step]"
+    using firstUpdate
+    unfolding UPDATE1_step_def
+    by (metis append_butlast_last_id)
+  then show ?thesis
+    using reachableFromInitI that
+    unfolding UPDATE1_step_def
+    by (smt (verit, best) \<open>\<And>thesis. (\<And>steps. stepsInit = steps @ [UPDATE1_step] \<Longrightarrow> thesis) \<Longrightarrow> thesis\<close> \<open>stepsInit = steps @ [UPDATE1_step]\<close> append.right_neutral butlast.simps(2) butlast_append executeStep.simps(3) list.distinct(1) reachableFrom.cases reachableFromAppend reachableFromCons')
+qed
+
+lemma getLastStateBContractsU:
+  assumes "callUpdate contractsInit (stateOracleAddressB contractsInit bridgeAddress) blockU blockNumU stateRootInit = (Success, contractsU)"
+  shows "getLastStateB contractsU bridgeAddress = stateRootInit"
+  using assms
+  using callUpdateIBridge callUpdateLastState 
+  by presburger
+
+lemma generateStateRootInit:
+  shows "generateStateRoot contractsInit = stateRootInit"
+proof-
+  obtain blockU blockNumU contractsU
+    where "callUpdate contractsInit (stateOracleAddressB contractsInit bridgeAddress) blockU blockNumU stateRootInit = (Success, contractsU)"
+    by (meson obtainContractsU)
+  then show ?thesis
+    using updateSuccess 
+    by blast
+qed
+
+lemma getLastStateBContractsUNonZero:
+  shows "getLastStateB contractsI bridgeAddress \<noteq> 0"
+  by (metis lastStateNonZero reachableFromBridgeStateOracle firstUpdate last_in_set reachableFromInitI updatesNonZeroInit)
+
+end
+
+context InitFirstUpdate
+begin
 
 text \<open>Before every successful claim, a deposit must have been made\<close>
 theorem depositBeforeClaim:
-  \<comment> \<open>The operation starts from an initial state that is properly setup, but all data is still empty\<close>
-  assumes "properSetup initContracts tokenDepositAddress bridgeAddress"
-  assumes "getDeposit (the (tokenDepositState initContracts tokenDepositAddress)) ID = 0"
-  assumes "getLastStateB initContracts bridgeAddress = 0"
-
-  \<comment> \<open>From the initial state, the state in which claim is successful is reached\<close>
-  assumes "reachableFrom initContracts contracts steps"
-  \<comment> \<open>There has been at least one state update\<close>
-  assumes update:
-          "let stateOracleAddress = stateOracleAddressB initContracts bridgeAddress
-            in UPDATE stateOracleAddress stateRoot \<in> set steps"
   \<comment> \<open>Claim was successful\<close>
-  assumes "callClaim contracts bridgeAddress msg ID token amount proof = (Success, contracts')"
-
-  (* NOTE: additional assumptions *)
-  \<comment> \<open>Updates never set zero state root\<close>
-  assumes "updatesNonZero steps"
-  \<comment> \<open>hash of the transaction is non-zero\<close>
-  assumes "hash3 (sender msg) token amount \<noteq> 0"
-  \<comment> \<open>hash function is injective\<close>
-  assumes hash3_inj
-
+  assumes "callClaim contractsI bridgeAddress msg ID token amount proof = (Success, contractsClaim)"
   \<comment> \<open>The correct deposit must have happened\<close>
-  shows "DEPOSIT tokenDepositAddress (sender msg) ID token amount \<in> set steps"
+  shows "DEPOSIT tokenDepositAddress (sender msg) ID token amount \<in> set stepsInit"
 proof-
-  define stateOracleAddress where "stateOracleAddress = stateOracleAddressB initContracts bridgeAddress"
-
-  have "lastState (the (stateOracleState contracts stateOracleAddress)) \<noteq> 0"
-    using \<open>reachableFrom initContracts contracts steps\<close> update \<open>updatesNonZero steps\<close> 
-    using lastStateNonZero stateOracleAddress_def
-    by force
-
+  define stateOracleAddress where "stateOracleAddress = stateOracleAddressB contractsInit bridgeAddress"
+  have "lastState (the (stateOracleState contractsInit stateOracleAddress)) = 0"
+    using lastStateBZero stateOracleAddress_def by blast
   moreover
-
-  have "lastState (the (stateOracleState initContracts stateOracleAddress)) = 0"
-    using assms lastStateNonZero stateOracleAddress_def
-    by force
-
-  ultimately 
-
-  obtain contractsU contractsU' block blockNum steps1 steps2 stateRoot' where
-    "reachableFrom initContracts contractsU steps1"
+  have "lastState (the (stateOracleState contractsI stateOracleAddress)) \<noteq> 0"
+    by (metis getLastStateBContractsUNonZero reachableFromBridgeStateOracle reachableFromInitI stateOracleAddress_def)
+  ultimately
+  obtain contractsU contractsU' block blockNum steps1 steps2 stateRoot' where *:
+    "reachableFrom contractsInit contractsU steps1"
     "stateRoot' = generateStateRoot contractsU"
     "callUpdate contractsU stateOracleAddress block blockNum stateRoot' = (Success, contractsU')"
-    "reachableFrom contractsU' contracts steps2"
+    "reachableFrom contractsU' contractsI steps2"
     "\<nexists>stateRoot'. UPDATE stateOracleAddress stateRoot' \<in> set steps2"
-    "set steps1 \<subseteq> set steps"
-    using lastUpdateHappened[OF \<open>reachableFrom initContracts contracts steps\<close>, of stateOracleAddress]
+    "set steps1 \<subseteq> set stepsInit"
+    using lastUpdateHappened[OF reachableFromInitI, of stateOracleAddress]
     by auto
-  
-  then have "getDeposit (the (tokenDepositState contractsU tokenDepositAddress)) ID = hash3 (sender msg) token amount"
-    using assms callClaimGetDeposit 
+
+  interpret LastUpdate': LastUpdate where 
+    contractsLastUpdate'=contractsU and
+    contractsLastUpdate=contractsU' and
+    contractsLU=contractsI and
+    stepsNoUpdate=steps2 and
+    blockLU=block and
+    blockNumLU=blockNum and
+    stateRoot=stateRoot'
+  proof
+    show "properSetup contractsU tokenDepositAddress bridgeAddress"
+      using \<open>reachableFrom contractsInit contractsU steps1\<close> assms(1) 
+      by auto
+  next
+    show "let stateOracleAddress = stateOracleAddressB contractsU bridgeAddress
+           in callUpdate contractsU stateOracleAddress block blockNum stateRoot' = (Success, contractsU')"
+      by (metis "*"(1) "*"(3) reachableFromBridgeStateOracle stateOracleAddress_def)
+  next
+    show "reachableFrom contractsU' contractsI steps2"
+      by fact
+  next
+    show "let stateOracleAddress = stateOracleAddressB contractsU' bridgeAddress
+           in \<nexists>stateRoot'. UPDATE stateOracleAddress stateRoot' \<in> set steps2"
+      by (metis "*"(4) "*"(5) reachableFromBridgeStateOracle reachableFromInitI stateOracleAddress_def)
+  qed
+
+  have "getDeposit (the (tokenDepositState contractsU tokenDepositAddress)) ID = hash3 (sender msg) token amount"
+    using assms LastUpdate'.callClaimGetDeposit
     by (smt (verit, best) reachableFromBridgeStateOracle callUpdateITokenDeposit properSetupReachable stateOracleAddress_def)
   then show ?thesis
     using hashWrittenOnlyByDeposit
-    using assms 
-    using \<open>reachableFrom initContracts contractsU steps1\<close> \<open>set steps1 \<subseteq> set steps\<close> by blast
+    using depositsEmpty assms
+    using \<open>reachableFrom contractsInit contractsU steps1\<close> \<open>set steps1 \<subseteq> set stepsInit\<close>
+    by blast
 qed
 
+end
+
+context StrongHashProofVerifier
+begin
+
 (* ------------------------------------------------------------------------------------ *)
-
+(*
+               deposit           [steps]            claim
+    contractsD   \<rightarrow>   contractsD'  \<rightarrow>*   contractsC    \<rightarrow>   contractsC'
+    properSetup                  UPDATE
+*)
 text \<open>Only user who made the deposit can make a successful claim with the same ID\<close>
-
 lemma onlyDepositorCanClaim:
   \<comment> \<open>deposit is done a properly configured state state\<close>
   assumes "properSetup contractsD tokenDepositAddress bridgeAddress"
   assumes deposit: "callDeposit contractsD tokenDepositAddress block msg ID token amount = (Success, contractsD')"
+  \<comment> \<open>after a while a  claim is made\<close>
+  assumes "reachableFrom contractsD' contractsC steps"
+  assumes claim: "callClaim contractsC bridgeAddress msg' ID token' amount' proof = (Success, contractsC')"
+  \<comment> \<open>in the meantime a state oracle update is made\<close>
+  assumes update: "UPDATE (stateOracleAddressB contractsD bridgeAddress) stateRoot \<in> set steps"
+
   (* FIXME: amount must be the same as the value of the message - this assumption can be removed when the definition of executeStep is changed *)
   assumes "val msg = amount"
-
-  \<comment> \<open>in some state after the deposit a state oracle update is made\<close>
-  assumes "reachableFrom contractsD' contractsU steps2"
-  assumes update: "callUpdate contractsU (stateOracleAddressB contractsU bridgeAddress) block blockNum stateRoot = (Success, contractsU')"
-
-  \<comment> \<open>in some state after the update a successfull claim is made with the same ID\<close>
-  assumes "reachableFrom contractsU' contractsC steps3"
-  assumes claim: "callClaim contractsC bridgeAddress msg' ID token' amount' proof = (Success, contractsC')"
-
-  (* NOTE: additional assumptions *)
-  \<comment> \<open>transaction hashes are not zero\<close>
-  assumes "hash3 (sender msg) token amount \<noteq> 0"
-  assumes "hash3 (sender msg') token' amount' \<noteq> 0"
-  \<comment> \<open>the hash function is injective\<close>
-  assumes hash3_inj
 
   shows "sender msg = sender msg'" "token = token'" "amount = amount'"
 proof-
@@ -618,584 +578,118 @@ proof-
 
   define stateOracleAddress where "stateOracleAddress = stateOracleAddressB contractsD bridgeAddress"
 
+  let ?update = "UPDATE (stateOracleAddressB contractsD bridgeAddress) stateRoot"
+
+  obtain steps1 steps2 contractsU contractsU' blockU blockNumU where *:
+   "reachableFrom contractsD' contractsU steps2"
+   "executeStep contractsU blockU blockNumU ?update = (Success, contractsU')"
+   "reachableFrom contractsU' contractsC steps1"
+    using reachableFromStepInSteps[OF \<open>reachableFrom contractsD' contractsC steps\<close> update]
+    by (smt (verit, ccfv_threshold) assms(3) in_set_conv_decomp_last reachableFromAppend reachableFromCons' update)
+
   let ?d = "DEPOSIT tokenDepositAddress (sender msg) ID token amount"
   let ?u = "UPDATE stateOracleAddress stateRoot"
-  let ?steps = "steps2 @ [?d]"
 
-  obtain contractsUx contractsU'x blockx blockNumx steps1x steps2x stateRootx where
+  have "stateOracleAddressB contractsD' bridgeAddress = stateOracleAddressB contractsD bridgeAddress"
+    using Hash.callDepositIBridge deposit 
+    by presburger
+
+  have **: "callUpdate contractsU stateOracleAddress blockNumU blockU stateRoot = (Success, contractsU')"
+    using \<open>executeStep contractsU blockU blockNumU (UPDATE (stateOracleAddressB contractsD bridgeAddress) stateRoot) = (Success, contractsU')\<close> 
+    unfolding stateOracleAddress_def 
+    by auto
+
+  obtain contractsUx contractsU'x blockx blockNumx steps1x steps2x stateRootx where *:
     "reachableFrom contractsD' contractsUx steps1x"
     "stateRootx = generateStateRoot contractsUx"
     "callUpdate contractsUx stateOracleAddress blockx blockNumx stateRootx = (Success, contractsU'x)"
     "reachableFrom contractsU'x contractsC steps2x"
     "\<nexists>stateRoot'. UPDATE stateOracleAddress stateRoot' \<in> set steps2x"
-    using lastUpdateHappened'[of contractsD' contractsU _ stateOracleAddress block blockNum stateRoot contractsU' contractsC steps3] update
-    using \<open>reachableFrom contractsD' contractsU steps2\<close>
-    using \<open>reachableFrom contractsU' contractsC steps3\<close>
-    by (metis callDepositIBridge deposit reachableFromBridgeStateOracle stateOracleAddress_def)
+    using lastUpdateHappened'[OF \<open>reachableFrom contractsD' contractsU steps2\<close> ** \<open>reachableFrom contractsU' contractsC steps1\<close>]
+    by metis
 
-  have "getDeposit (the (tokenDepositState contractsU'x tokenDepositAddress)) ID = hash3 (sender msg') token' amount'"
-  proof (rule callClaimGetDeposit)
-    show "callClaim contractsC bridgeAddress msg' ID token' amount' proof = (Success, contractsC')"
-      by fact
+  interpret LastUpdate': LastUpdate where
+     contractsLastUpdate'=contractsUx and 
+     contractsLastUpdate=contractsU'x and
+     contractsLU=contractsC and
+     stepsNoUpdate=steps2x and
+     blockLU=blockx and
+     blockNumLU=blockNumx and
+     stateRoot = stateRootx
+  proof
+    show "properSetup contractsUx tokenDepositAddress bridgeAddress"
+      using \<open>reachableFrom contractsD' contractsUx steps1x\<close> assms(1) deposit by auto
   next
     show "let stateOracleAddress = stateOracleAddressB contractsUx bridgeAddress
-           in callUpdate contractsUx stateOracleAddress blockx blockNumx stateRootx =
-              (Success, contractsU'x)"
-      using \<open>callUpdate contractsUx stateOracleAddress blockx blockNumx stateRootx = (Success, contractsU'x)\<close>
-      using \<open>reachableFrom contractsD' contractsUx steps1x\<close>
-      by (metis Hash.callDepositIBridge deposit reachableFromBridgeStateOracle stateOracleAddress_def)
-  next
-    show "properSetup contractsUx tokenDepositAddress bridgeAddress"
-      using \<open>reachableFrom contractsD' contractsUx steps1x\<close> 
-      using \<open>properSetup contractsD tokenDepositAddress bridgeAddress\<close> 
-      using properSetupReachable callDepositProperSetup deposit
-      by blast
+           in callUpdate contractsUx stateOracleAddress blockx blockNumx stateRootx = (Success, contractsU'x)"
+      using * \<open>stateOracleAddressB contractsD' bridgeAddress = stateOracleAddressB contractsD bridgeAddress\<close> 
+      unfolding stateOracleAddress_def
+      by simp
   next
     show "reachableFrom contractsU'x contractsC steps2x"
       by fact
   next
-    show "let stateOracleAddress = stateOracleAddressB contractsUx bridgeAddress
+    show "let stateOracleAddress = stateOracleAddressB contractsU'x bridgeAddress
            in \<nexists>stateRoot'. UPDATE stateOracleAddress stateRoot' \<in> set steps2x"
-      using \<open>\<nexists>stateRoot'. UPDATE stateOracleAddress stateRoot' \<in> set steps2x\<close>
-             \<open>reachableFrom contractsD' contractsUx steps1x\<close> stateOracleAddress_def
-      by (metis callDepositIBridge deposit reachableFromBridgeStateOracle)
+      using * \<open>stateOracleAddressB contractsD' bridgeAddress = stateOracleAddressB contractsD bridgeAddress\<close>
+      unfolding stateOracleAddress_def
+      by simp
   qed
+
+  have "getDeposit (the (tokenDepositState contractsUx tokenDepositAddress)) ID = hash3 (sender msg') token' amount'"
+    using LastUpdate'.callClaimGetDeposit[OF claim]
+    by simp
 
   have "hash3 (sender msg) token amount = hash3 (sender msg') token' amount'"
     using reachableFromGetDeposit
-    using \<open>getDeposit (the (tokenDepositState contractsD' tokenDepositAddress)) ID = hash3 (sender msg) token amount\<close> \<open>getDeposit (the (tokenDepositState contractsU'x tokenDepositAddress)) ID = hash3 (sender msg') token' amount'\<close>
+    using \<open>getDeposit (the (tokenDepositState contractsD' tokenDepositAddress)) ID = hash3 (sender msg) token amount\<close> 
+    using \<open>getDeposit (the (tokenDepositState contractsUx tokenDepositAddress)) ID = hash3 (sender msg') token' amount'\<close>
     using \<open>callUpdate contractsUx stateOracleAddress blockx blockNumx stateRootx = (Success, contractsU'x)\<close>
-    using \<open>hash3 (sender msg) token amount \<noteq> 0\<close>  \<open>hash3 (sender msg') token' amount' \<noteq> 0\<close>
+    using hash3_nonzero
     using \<open>reachableFrom contractsD' contractsUx steps1x\<close>
     by (metis callUpdateITokenDeposit)
-
   then show "sender msg = sender msg'" "token = token'" "amount = amount'"
-    using \<open>hash3_inj\<close>
+    using hash3_inj
     unfolding hash3_inj_def
     by metis+
 qed
 
-(* ------------------------------------------------------------------------------------ *)
+end
+
+
+context Init
+begin
+
+(*
+                  [steps]              cancel
+  contractsInit     \<rightarrow>*      contracts   \<rightarrow>   contracts'
+  properSetup    DEPOSIT?
+  getDeposit=0
+*)
 
 text \<open>Cancel deposit can succeed only if there was a previous successful deposit with the same ID\<close>
 theorem cancelDepositOnlyAfterDeposit:
-  \<comment> \<open>contracts start working from a properly setup initial state\<close>
-  assumes "properSetup initContracts tokenDepositAddress bridgeAddress"
-  assumes "getDeposit (the (tokenDepositState initContracts tokenDepositAddress)) ID = 0"
-
-  \<comment> \<open>at some later state cancel deposit succeeded\<close>
-  assumes "reachableFrom initContracts contracts steps"
-  assumes cancel: "callCancelDepositWhileDead contracts tokenDepositAddress msg block ID token amount proof = (Success, contracts')"
-
-  (* NOTE: additional assumptions *)
-  \<comment> \<open>hash value of the transaction is not zero\<close>
-  assumes "hash3 (sender msg) token amount \<noteq> 0"
-  \<comment> \<open>the hash function is injective\<close>
-  assumes hash3_inj
-
+  assumes cancel: 
+    "callCancelDepositWhileDead contractsI tokenDepositAddress msg block ID token amount proof = 
+     (Success, contracts')"
   \<comment> \<open>there must had been a previous deposit with the same ID\<close>
-  shows "DEPOSIT tokenDepositAddress (sender msg) ID token amount \<in> set steps"
+  shows "DEPOSIT tokenDepositAddress (sender msg) ID token amount \<in> set stepsInit"
 proof-
-  have "getDeposit (the (tokenDepositState contracts tokenDepositAddress)) ID = hash3 (sender msg) token amount"
+  have "getDeposit (the (tokenDepositState contractsI tokenDepositAddress)) ID = hash3 (sender msg) token amount"
     using cancel
     unfolding callCancelDepositWhileDead_def cancelDepositWhileDead_def
     by (simp add: Let_def split: option.splits prod.splits if_split_asm)
   then show ?thesis
-    using assms hashWrittenOnlyByDeposit
+    using assms hashWrittenOnlyByDeposit depositsEmpty reachableFromInitI
     by blast
 qed
 
-text \<open>When the bridge dies the dead state is set to the state root set in the last update\<close>
-lemma deadStateLastState:
-  assumes "reachableFrom contracts contracts' steps"
-  assumes "properSetup contracts tokenDepositAddress bridgeAddress"
-  assumes noUpdate:
-          "let stateOracleAddress = stateOracleAddressB contracts bridgeAddress
-            in \<nexists> stateRoot'. UPDATE stateOracleAddress stateRoot' \<in> set steps"
-  assumes "\<not>bridgeDead contracts tokenDepositAddress"
-  assumes "bridgeDead contracts' tokenDepositAddress"
-  assumes "let stateOracleAddress = stateOracleAddressB contracts bridgeAddress
-            in callLastState contracts stateOracleAddress = (Success, stateRoot)"
-  shows "deadState (the (tokenDepositState contracts' tokenDepositAddress)) = stateRoot"
-  using assms
-proof (induction contracts contracts' steps rule: reachableFrom.induct)
-  case (reachableFrom_base contracts)
-  then show ?case
-    by blast
-next
-  case (reachableFrom_step steps contracts'' contracts contracts' blockNum block step)
-  show ?case
-  proof (cases "deadState (the (tokenDepositState contracts' tokenDepositAddress)) \<noteq> 0")
-    case True
-    then show ?thesis
-      using reachableFrom_step
-      apply (cases step)
-      apply (metis callDepositInDeadState executeStep.simps(1) list.set_intros(2))
-      apply simp
-      apply (metis callUpdateDeadState executeStep.simps(3) list.set_intros(2))
-      apply (metis callCancelDepositWhileDeadInDeadState executeStep.simps(4) list.set_intros(2))
-      apply (metis callWithdrawWhileDeadInDeadState executeStep.simps(5) list.set_intros(2))
-      done
-  next
-    case False
-    show ?thesis
-    proof (cases step)
-      case (DEPOSIT address' caller' ID' token' amount')
-      show ?thesis
-      proof (cases "address' = tokenDepositAddress")
-        case False
-        then show ?thesis
-          using reachableFrom_step
-          by (metis DEPOSIT callDepositOtherAddress executeStep.simps(1) list.set_intros(2))
-      next
-        case True
-        show ?thesis
-        proof (rule callDepositSetsDeadState)
-          show "getLastStateTD contracts' tokenDepositAddress = stateRoot"
-            using reachableFrom_step.prems reachableFrom_step.hyps
-            by (smt (verit, ccfv_threshold) noUpdateLastState callLastState callLastStateI list.set_intros(2) prod.exhaust_sel properSetupReachable properSetup_def reachableFromBridgeStateOracle)
-        next
-          show "deadState (the (tokenDepositState contracts'' tokenDepositAddress)) \<noteq> 0"
-            by fact
-        next
-          show "callDeposit contracts' tokenDepositAddress block (message caller' amount') ID' token' amount' =
-                (Success, contracts'')"
-            using reachableFrom_step DEPOSIT \<open>address' = tokenDepositAddress\<close>
-            by simp
-        qed
-      qed
-    next
-      case (CLAIM address' caller' ID' token' amount' proof')
-      then show ?thesis
-        using reachableFrom_step
-        by simp
-    next
-      case (UPDATE address' stateRoot')
-      then show ?thesis
-        using reachableFrom_step
-        by (metis False callUpdateDeadState executeStep.simps(3))
-    next
-      case (CANCEL address' caller' ID' token' amount' proof')
-      show ?thesis
-      proof (cases "address' = tokenDepositAddress")
-        case False
-        then show ?thesis
-          using reachableFrom_step
-          by (metis CANCEL callCancelDepositWhileDeadOtherAddress executeStep.simps(4) list.set_intros(2))
-      next
-        case True
-        have "deadState (the (tokenDepositState contracts'' tokenDepositAddress)) = getLastStateTD contracts' tokenDepositAddress"
-        proof (rule callCancelDepositWhileDeadSetsDeadState)
-          show "\<not> bridgeDead contracts' tokenDepositAddress"
-            by fact
-        next
-          show "callCancelDepositWhileDead contracts' tokenDepositAddress (message caller' 0) block ID' token' amount' proof' =
-               (Success, contracts'')"
-            using CANCEL reachableFrom_step.prems reachableFrom_step.hyps True
-            by auto
-        qed
-        then show ?thesis
-          using reachableFrom_step.prems reachableFrom_step.hyps
-          by (smt (verit, ccfv_threshold) noUpdateLastState callLastState callLastStateI list.set_intros(2) prod.exhaust_sel properSetupReachable properSetup_def reachableFromBridgeStateOracle)
-      qed
-    next
-      case (WITHDRAW address' caller' token' amount' proof')
-      show ?thesis
-      proof (cases "address' = tokenDepositAddress")
-        case False
-        then show ?thesis
-          using reachableFrom_step
-          by (metis callWithdrawWhileDeadOtherAddress WITHDRAW executeStep.simps(5) list.set_intros(2))
-      next
-        case True
-        have "deadState (the (tokenDepositState contracts'' tokenDepositAddress)) = getLastStateTD contracts' tokenDepositAddress"
-        proof (rule callWithdrawWhileDeadSetsDeadState)
-          show "\<not> bridgeDead contracts' tokenDepositAddress"
-            by fact
-        next
-          show "callWithdrawWhileDead contracts' tokenDepositAddress (message caller' 0) block token' amount' proof' =
-               (Success, contracts'')"
-            using WITHDRAW reachableFrom_step.prems reachableFrom_step.hyps True
-            by auto
-        qed
-        then show ?thesis
-          using reachableFrom_step.prems reachableFrom_step.hyps
-          by (smt (verit, ccfv_threshold) noUpdateLastState callLastState callLastStateI list.set_intros(2) prod.exhaust_sel properSetupReachable properSetup_def reachableFromBridgeStateOracle)
-      qed
-    qed
-  qed
-qed
+end
 
-lemma deadStateLastStateRoot:
-  assumes "properSetup initContracts tokenDepositAddress bridgeAddress"
-  assumes "reachableFrom initContracts contracts steps"
-  \<comment> \<open>The last update that happened when the bridge was still alive\<close>
-  assumes update:
-          "let stateOracleAddress = BridgeState.stateOracle (the (bridgeState initContracts bridgeAddress))
-            in callUpdate contracts stateOracleAddress block blockNum stateRoot = (Success, contracts')"
-  assumes "stateRoot \<noteq> 0" (* NOTE: additional assumption *)
-  assumes "deadState (the (tokenDepositState contracts tokenDepositAddress)) = 0"
-  \<comment> \<open>There were no updates since then\<close>
-  assumes "reachableFrom contracts' contracts'' steps'"
-  assumes noUpdate: "let stateOracleAddress = BridgeState.stateOracle (the (bridgeState initContracts bridgeAddress))
-            in \<nexists> stateRoot'. UPDATE stateOracleAddress stateRoot' \<in> set steps'"
-  \<comment> \<open>The bridge is dead\<close>
-  assumes status: "let stateTokenDeposit = the (tokenDepositState contracts'' tokenDepositAddress)
-                    in getDeadStatus contracts'' stateTokenDeposit block' = (Success, True, stateTokenDeposit')"
+context HashProofVerifier
+begin
 
-  shows "generateStateRoot contracts = deadState stateTokenDeposit'"
-proof-
-  define stateBridge where "stateBridge = the (bridgeState contracts'' bridgeAddress)"
-  define stateStateOracle where "stateStateOracle = the (stateOracleState contracts'' (BridgeState.stateOracle stateBridge))"
-  define stateTokenDeposit where "stateTokenDeposit = the (tokenDepositState contracts'' tokenDepositAddress)"
-  define stateERC20 where "stateERC20 = the (ERC20state contracts' token)"
-
-  have sOB: "BridgeState.stateOracle stateBridge = BridgeState.stateOracle (the (bridgeState initContracts bridgeAddress))"
-    using assms
-    unfolding stateBridge_def
-    by simp
-
-  have "properSetup contracts' tokenDepositAddress bridgeAddress"
-    using assms
-    by (meson callUpdateProperSetup properSetupReachable)
-
-  from update have "generateStateRoot contracts = stateRoot"
-    using updateSuccess
-    by simp
-
-  have "lastState stateStateOracle = stateRoot"
-    using assms
-    by (metis (no_types, lifting) callUpdateLastState noUpdateLastState sOB stateStateOracle_def)
-  then have "getLastStateB contracts'' bridgeAddress = stateRoot"
-    using stateBridge_def stateStateOracle_def
-    by argo
-  then have "getLastStateTD contracts'' tokenDepositAddress = stateRoot"
-    using assms properSetup_stateOracleAddress update
-    by auto
-
-  have "deadState stateTokenDeposit' = stateRoot"
-  proof (cases "bridgeDead contracts'' tokenDepositAddress")
-    case True 
-    have "deadState (the (tokenDepositState contracts'' tokenDepositAddress)) = stateRoot"
-    proof (rule deadStateLastState)
-      show "reachableFrom contracts' contracts'' steps'"
-        by fact
-    next
-      show "properSetup contracts' tokenDepositAddress bridgeAddress" 
-        by fact 
-    next
-      show "let stateOracleAddress = stateOracleAddressB contracts' bridgeAddress
-             in \<nexists>stateRoot'. UPDATE stateOracleAddress stateRoot' \<in> set steps'"
-        using \<open>reachableFrom contracts' contracts'' steps'\<close>
-        by (metis noUpdate reachableFromBridgeStateOracle sOB stateBridge_def)
-    next
-      show "\<not> bridgeDead contracts' tokenDepositAddress"
-        using \<open>deadState (the (tokenDepositState contracts tokenDepositAddress)) = 0\<close> update
-        using callUpdateDeadState
-        by presburger
-    next
-      show "bridgeDead contracts'' tokenDepositAddress"
-        by fact
-    next
-      show "let stateOracleAddress = stateOracleAddressB contracts' bridgeAddress
-             in callLastState contracts' stateOracleAddress = (Success, stateRoot)"
-        using \<open>properSetup contracts' tokenDepositAddress bridgeAddress\<close> 
-              \<open>reachableFrom contracts' contracts'' steps'\<close>
-        by (smt (verit, best) callLastState_def callUpdateLastState option.case_eq_if properSetup_def reachableFromBridgeStateOracle sOB stateBridge_def update)
-    qed
-    then show ?thesis
-      using \<open>stateRoot \<noteq> 0\<close> 
-      using getDeadStatusInDeadState status
-      unfolding Let_def stateTokenDeposit_def
-      by blast
-  next
-    case False
-    then have "deadState stateTokenDeposit' = stateRoot"
-      using getDeadStatusSetsDeadState status
-      using \<open>getLastStateTD contracts'' tokenDepositAddress = stateRoot\<close>
-      unfolding stateTokenDeposit_def
-      by fastforce
-    then show ?thesis
-      by simp
-  qed
-
-  then show ?thesis
-    using \<open>generateStateRoot contracts = stateRoot\<close>
-    by simp
-qed
-
-
-text \<open>If cancel deposit succeeds, then the bridge is dead and 
-      there was no claim previous to the state in which the bridge died\<close>
-theorem cancelDepositNoClaim:
-  assumes "properSetup initContracts tokenDepositAddress bridgeAddress"
-  assumes "reachableFrom initContracts contracts steps"
-  \<comment> \<open>The last update that happened when the bridge was still alive\<close>
-  assumes update:
-          "let stateOracleAddress = BridgeState.stateOracle (the (bridgeState initContracts bridgeAddress))
-            in callUpdate contracts stateOracleAddress block blockNum stateRoot = (Success, contracts')"
-  assumes "stateRoot \<noteq> 0" (* NOTE: additional assumption *)
-  assumes "deadState (the (tokenDepositState contracts tokenDepositAddress)) = 0"
-  \<comment> \<open>There were no updates since then\<close>
-  assumes "reachableFrom contracts' contracts'' steps'"
-  assumes noUpdate: "let stateOracleAddress = BridgeState.stateOracle (the (bridgeState initContracts bridgeAddress))
-            in \<nexists> stateRoot'. UPDATE stateOracleAddress stateRoot' \<in> set steps'"
-  \<comment> \<open>Cancel deposit succeded\<close>
-  assumes cancel:
-          "callCancelDepositWhileDead contracts'' tokenDepositAddress msg block' ID token amount proof = (Success, contracts''')"
-  \<comment> \<open>Claim did not happen before that last update\<close>
-  shows "\<nexists> proof. CLAIM bridgeAddress (sender msg) ID token amount proof \<in> set steps"
-proof (rule ccontr)
-  assume "\<not> ?thesis"
-  then obtain p where *: "CLAIM bridgeAddress (sender msg) ID token amount p \<in> set steps"
-    by auto
-  have "getClaim (the (bridgeState contracts bridgeAddress)) ID = True"
-    using \<open>reachableFrom initContracts contracts steps\<close> *
-    by (simp add: claimStepSetsClaim)
-
-  moreover
-
-  define stateTokenDeposit where "stateTokenDeposit = the (tokenDepositState contracts'' tokenDepositAddress)"
-  define stateTokenDeposit' where "stateTokenDeposit' = snd (snd (getDeadStatus contracts'' stateTokenDeposit block'))"
-  define stateBridge where "stateBridge = the (bridgeState contracts'' bridgeAddress)"
-
-  have bD: "TokenDepositState.bridge stateTokenDeposit = bridgeAddress"
-    using assms
-    unfolding stateTokenDeposit_def
-    by (meson callUpdateProperSetup properSetupReachable properSetup_def)
-
-  have status: "getDeadStatus contracts'' stateTokenDeposit block' = (Success, True, stateTokenDeposit')" 
-    using cancel
-    unfolding callCancelDepositWhileDead_def cancelDepositWhileDead_def stateTokenDeposit_def stateTokenDeposit'_def lastValidState_def
-    by (simp add: Let_def split: option.splits prod.splits if_split_asm)
-
-  then have lVS: "lastValidState contracts'' stateTokenDeposit' = (Success, deadState stateTokenDeposit')" 
-    using cancel
-    using callLastState getDeadStatusTrueDeadState assms
-    unfolding callCancelDepositWhileDead_def cancelDepositWhileDead_def stateTokenDeposit_def stateTokenDeposit'_def lastValidState_def
-    by (smt (verit, ccfv_SIG) deadStateLastStateRoot noUpdate update updateSuccess)
-    
-  then have vCP: "callVerifyClaimProof contracts'' (TokenDepositState.proofVerifier stateTokenDeposit') (bridge stateTokenDeposit') ID
-                  (deadState stateTokenDeposit') proof = Success"
-    using cancel
-    unfolding callCancelDepositWhileDead_def cancelDepositWhileDead_def stateTokenDeposit_def stateTokenDeposit'_def lastValidState_def
-    by (simp add: Let_def split: option.splits prod.splits if_split_asm)
-    
-  have "generateStateRoot contracts = deadState stateTokenDeposit'"
-    using assms status
-    by (metis deadStateLastStateRoot stateTokenDeposit_def)
- 
-  from update have "generateStateRoot contracts = stateRoot"
-    using updateSuccess
-    by simp
-
-  have "getClaim (the (bridgeState contracts bridgeAddress)) ID = False"
-  proof (rule verifyClaimProofE)
-    show "generateStateRoot contracts = stateRoot"
-      by fact
-  next
-    show "verifyClaimProof () bridgeAddress ID stateRoot proof = True"
-      using status vCP bD \<open>generateStateRoot contracts = deadState stateTokenDeposit'\<close> \<open>generateStateRoot contracts = stateRoot\<close> 
-      unfolding callVerifyClaimProof_def stateTokenDeposit'_def stateTokenDeposit_def
-      by (auto split: option.splits prod.splits if_split_asm)
-  next
-    have "bridgeState contracts bridgeAddress \<noteq> None"
-      using assms
-      by (meson \<open>reachableFrom initContracts contracts steps\<close> properSetup_def reachableFromBridgeState)
-    then show "bridgeState contracts bridgeAddress = Some (the (bridgeState contracts bridgeAddress))"
-      by simp
-  qed
-
-  ultimately
-
-  show False
-    by simp
-qed
-
-
-text \<open>If withdrawal succeeds, then the bridge is dead and 
-      the user had the exact amount of tokens in the state in which the bridge died\<close>
-theorem withdrawSufficientBalance:
-  assumes "properSetup initContracts tokenDepositAddress bridgeAddress"
-  assumes "properToken initContracts tokenDepositAddress bridgeAddress token"
-  assumes "reachableFrom initContracts contracts steps"
-  \<comment> \<open>The last update that happened when the bridge was still alive\<close>
-  assumes update:
-          "let stateOracleAddress = BridgeState.stateOracle (the (bridgeState initContracts bridgeAddress))
-            in callUpdate contracts stateOracleAddress block blockNum stateRoot = (Success, contracts')"
-  assumes "stateRoot \<noteq> 0" (* NOTE: additional assumption *)
-  assumes "deadState (the (tokenDepositState contracts tokenDepositAddress)) = 0"
-  \<comment> \<open>There were no updates since then\<close>
-  assumes "reachableFrom contracts' contracts'' steps'"
-  assumes noUpdate: "let stateOracleAddress = BridgeState.stateOracle (the (bridgeState initContracts bridgeAddress))
-            in \<nexists> stateRoot'. UPDATE stateOracleAddress stateRoot' \<in> set steps'"
-  \<comment> \<open>Withdraw succeded\<close>
-  assumes withdraw:
-          "callWithdrawWhileDead contracts'' tokenDepositAddress msg block' token amount proof = (Success, contracts''')"
-  \<comment> \<open>Caller had sufficient balance\<close>
-  shows "callBalanceOf contracts token (sender msg) = (Success, amount)"
-proof-
-  have "properSetup contracts' tokenDepositAddress bridgeAddress"
-    using assms
-    by (meson callUpdateProperSetup properSetupReachable)
-
-  have "properToken contracts' tokenDepositAddress bridgeAddress token"
-    using assms
-    by (meson callUpdateProperToken properTokenReachable)
-
-  from update have "generateStateRoot contracts = stateRoot"
-    using updateSuccess
-    by simp
-
-  define stateTokenDeposit where "stateTokenDeposit = the (tokenDepositState contracts'' tokenDepositAddress)"
-  define stateTokenDeposit' where "stateTokenDeposit' = snd (snd (getDeadStatus contracts'' stateTokenDeposit block'))"
-  define stateERC20 where "stateERC20 = the (ERC20state contracts' token)"
- 
-  have status: "getDeadStatus contracts'' stateTokenDeposit block' = (Success, True, stateTokenDeposit')" and
-       vCP: "callVerifyBalanceProof contracts'' (TokenDepositState.proofVerifier stateTokenDeposit') token (sender msg) amount
-             (deadState stateTokenDeposit') proof = Success"
-    using withdraw
-    unfolding stateTokenDeposit_def stateTokenDeposit'_def
-    unfolding callWithdrawWhileDead_def withdrawWhileDead_def
-    by (simp_all add: Let_def split: option.splits prod.splits if_split_asm)
-
-  have "generateStateRoot contracts = deadState stateTokenDeposit'"
-    using assms status
-    by (metis deadStateLastStateRoot stateTokenDeposit_def)
-
-  have "ERC20state contracts token \<noteq> None"
-    using \<open>properToken contracts' tokenDepositAddress bridgeAddress token\<close> update
-    by (metis callUpdateIERC20 properToken_def)
-
-  have "balanceOf (the (ERC20state contracts token)) (sender msg) = amount"
-  proof (rule verifyBalanceProofE)
-    show "verifyBalanceProof () token (sender msg) amount stateRoot proof = True"
-      using vCP \<open>generateStateRoot contracts = stateRoot\<close> \<open>generateStateRoot contracts = deadState stateTokenDeposit'\<close>
-      unfolding callVerifyBalanceProof_def
-      by (simp split: option.splits if_split_asm)
-  next
-    show "generateStateRoot contracts = stateRoot"
-      by fact
-  next
-    show "ERC20state contracts token = Some (the (ERC20state contracts token))"
-      using \<open>ERC20state contracts token \<noteq> None\<close>
-      by simp
-  qed
-  then show ?thesis
-    using \<open>ERC20state contracts token \<noteq> None\<close>
-    unfolding callBalanceOf_def
-    by (auto split: option.splits)
-qed
-
-
-text \<open>If the user had some amount of tokens in the state in which the bridge died, 
-      he can withdraw that amount\<close>
-theorem sufficientBalanceCanWithdraw:
-  assumes "properSetup initContracts tokenDepositAddress bridgeAddress"
-  assumes "properToken initContracts tokenDepositAddress bridgeAddress token"
-
-  assumes "reachableFrom initContracts contracts steps"
-  \<comment> \<open>The last update that happened when the bridge was still alive\<close>
-  assumes update:
-          "let stateOracleAddress = BridgeState.stateOracle (the (bridgeState initContracts bridgeAddress))
-            in callUpdate contracts stateOracleAddress block blockNum stateRoot = (Success, contracts')"
-  assumes "stateRoot \<noteq> 0" (* NOTE: additional assumption *)
-  assumes "deadState (the (tokenDepositState contracts tokenDepositAddress)) = 0"
-  \<comment> \<open>There were no updates since then\<close>
-  assumes "reachableFrom contracts' contracts'' steps'"
-  assumes noUpdate: "let stateOracleAddress = BridgeState.stateOracle (the (bridgeState initContracts bridgeAddress))
-            in \<nexists> stateRoot'. UPDATE stateOracleAddress stateRoot' \<in> set steps'"
-  \<comment> \<open>Caller had sufficient balance\<close>
-  assumes "callBalanceOf contracts token (sender msg) = (Success, amount)"
-
-  \<comment> \<open>Caller has not yet withdrawn his balance\<close>
-  assumes notWithdrawn: "getTokenWithdrawn (the (tokenDepositState contracts'' tokenDepositAddress)) (hash2 (sender msg) token) = False"
-
-  \<comment> \<open>The bridge is dead\<close>
-  assumes dead: "deadState (the (tokenDepositState contracts'' tokenDepositAddress)) \<noteq> 0"
-
-  \<comment> \<open>Sender is not the bridge itself\<close>
-  assumes "tokenDepositAddress \<noteq> sender msg"
-
-  \<comment> \<open>Withdraw succedes\<close>
-  shows "fst (callWithdrawWhileDead contracts'' tokenDepositAddress msg block' token amount (generateBalanceProof contracts token (sender msg) amount)) = Success"
-proof-
-  define stateTokenDeposit where "stateTokenDeposit = the (tokenDepositState contracts'' tokenDepositAddress)"
-  define stateTokenDeposit' where "stateTokenDeposit' = snd (snd (getDeadStatus contracts'' stateTokenDeposit block'))"
-
-  have proper: "properSetup contracts tokenDepositAddress bridgeAddress"
-               "properToken contracts tokenDepositAddress bridgeAddress token"
-    using assms
-    by (meson properSetupReachable, meson properTokenReachable)
-  then have proper'': "properSetup contracts'' tokenDepositAddress bridgeAddress"
-                      "properToken contracts'' tokenDepositAddress bridgeAddress token"
-    using assms
-    by (meson callUpdateProperSetup properSetupReachable update, meson callUpdateProperToken properTokenReachable update)
-
-  have tds: "tokenDepositState contracts'' tokenDepositAddress \<noteq> None"
-    using proper''
-    by (metis properSetup_def)
-
-  have dead: "getDeadStatus contracts'' stateTokenDeposit block' = (Success, True, stateTokenDeposit')"
-    using dead
-    unfolding stateTokenDeposit_def stateTokenDeposit'_def
-    unfolding getDeadStatus_def
-    by auto
-
-  have bp: "callVerifyBalanceProof contracts'' (TokenDepositState.proofVerifier stateTokenDeposit') token (sender msg) amount
-            (deadState stateTokenDeposit') (generateBalanceProof contracts token (sender msg) amount) = Success"
-  proof-
-    have "verifyBalanceProof () token (sender msg) amount (deadState stateTokenDeposit') (generateBalanceProof contracts token (sender msg) amount) = True"
-    proof (rule verifyBalanceProofI)
-      show "generateBalanceProof contracts token (sender msg) amount = generateBalanceProof contracts token (sender msg) amount"
-        by simp
-    next
-      show "generateStateRoot contracts = deadState stateTokenDeposit'"
-        using assms
-        by (metis dead deadStateLastStateRoot noUpdate stateTokenDeposit_def update)
-    next
-      show "ERC20state contracts token = Some (the (ERC20state contracts token))"
-        using proper
-        unfolding properToken_def Let_def
-        by simp
-    next
-      show "balanceOf (the (ERC20state contracts token)) (sender msg) = amount"
-        using \<open>callBalanceOf contracts token (sender msg) = (Success, amount)\<close>
-        using callBalanceOf
-        by blast
-    qed
-    moreover 
-    have "proofVerifierState contracts'' (TokenDepositState.proofVerifier stateTokenDeposit) \<noteq> None"
-      using proper''
-      unfolding properSetup_def stateTokenDeposit_def
-      by (simp add: Let_def)
-    then have "proofVerifierState contracts'' (TokenDepositState.proofVerifier stateTokenDeposit') \<noteq> None"
-      using dead getDeadStatusProofVerifier by presburger
-    ultimately show ?thesis
-      unfolding callVerifyBalanceProof_def
-      by (auto split: option.splits)
-  qed
-
-  have transfer: "fst (callSafeTransferFrom contracts'' token tokenDepositAddress (sender msg) amount) = Success"
-  proof (rule callSafeTransferFromI)
-    show "ERC20state contracts'' token = Some (the (ERC20state contracts'' token))"
-      using proper''
-      by (metis option.collapse properToken_def)
-  next
-    show "tokenDepositAddress \<noteq> sender msg"
-      by fact
-  next
-    show "amount \<le> balanceOf (the (ERC20state contracts'' token)) tokenDepositAddress"
-      using \<open>callBalanceOf contracts token (sender msg) = (Success, amount)\<close>
-      sorry      
-  qed
-
-  show ?thesis
-    using tds dead bp transfer notWithdrawn
-    unfolding callWithdrawWhileDead_def withdrawWhileDead_def
-    unfolding stateTokenDeposit_def stateTokenDeposit'_def
-    by (auto simp add: Let_def split: option.splits prod.splits if_split)
-qed
+(* ------------------------------------------------------------------------------------ *)
 
 primrec DEPOSIT_amount where
   "DEPOSIT_amount (DEPOSIT address caller ID token amount) = amount"
@@ -1209,243 +703,166 @@ primrec WITHDRAW_amount where
 primrec CANCEL_amount where
   "CANCEL_amount (CANCEL address caller ID token amount proof) = amount"
 
-definition deposits where
-  "deposits address token steps = 
-   filter (\<lambda> step. case step of DEPOSIT address' caller ID token' amount \<Rightarrow> address = address' \<and> token = token' | _ \<Rightarrow> False) steps"
+fun isTokenDeposit :: "address \<Rightarrow> address \<Rightarrow> Step \<Rightarrow> bool" where
+  "isTokenDeposit address token (DEPOSIT address' caller ID token' amount) \<longleftrightarrow> address' = address \<and> token' = token"
+| "isTokenDeposit address token _ = False"
 
-definition depositedAmount where
-  "depositedAmount address token steps = 
-   sum_list (map DEPOSIT_amount (deposits address token steps))"
+\<comment> \<open>All deposits of the given token on the given address\<close>
+definition tokenDeposits where
+  "tokenDeposits address token steps = filter (isTokenDeposit address token) steps"
 
-lemma depositedAmountCons [simp]:
-  shows "depositedAmount address token (DEPOSIT address caller ID token amount # steps) = 
-         amount + depositedAmount address token steps"
-  by (simp add: deposits_def depositedAmount_def)
+\<comment> \<open>Total amount of the given token deposited on the given address\<close>
+definition depositedTokenAmount where
+  "depositedTokenAmount address token steps = sum_list (map DEPOSIT_amount (tokenDeposits address token steps))"
 
-lemma depositedAmountConsOther [simp]:
+lemma depositedTokenAmountCons [simp]:
+  shows "depositedTokenAmount address token (DEPOSIT address caller ID token amount # steps) = 
+         amount + depositedTokenAmount address token steps"
+  by (simp add: tokenDeposits_def depositedTokenAmount_def)
+
+lemma depositedTokenAmountConsOther [simp]:
   assumes "address \<noteq> address' \<or> token \<noteq> token'"
-  shows "depositedAmount address token (DEPOSIT address' caller ID token' amount # steps) = 
-         depositedAmount address token steps"
+  shows "depositedTokenAmount address token (DEPOSIT address' caller ID token' amount # steps) = 
+         depositedTokenAmount address token steps"
   using assms
-  by (auto simp add: deposits_def depositedAmount_def)
+  by (auto simp add: tokenDeposits_def depositedTokenAmount_def)
 
-lemma depositedAmoutConsNonDeposit [simp]:
+lemma depositedTokenAmoutConsNonDeposit [simp]:
   assumes "\<nexists> address' caller' ID' token' amount'. step = DEPOSIT address' caller' ID' token' amount'"
-  shows "depositedAmount address token (step # steps) = depositedAmount address token steps"
+  shows "depositedTokenAmount address token (step # steps) = depositedTokenAmount address token steps"
   using assms 
-  unfolding depositedAmount_def deposits_def
+  unfolding depositedTokenAmount_def tokenDeposits_def
   by (cases step, auto)
 
+fun isTokenClaim where
+  "isTokenClaim address token (CLAIM address' caller ID token' amount proof) \<longleftrightarrow> address' = address \<and> token' = token"
+| "isTokenClaim address token _ = False"
 
+\<comment> \<open>All claims of a given token on the given bridge\<close>
+definition tokenClaims where 
+  "tokenClaims address token steps = 
+   filter (isTokenClaim address token) steps"
 
-definition claims where 
-  "claims address token steps = 
-   filter (\<lambda> step. case step of CLAIM address' caller ID token' amount proof \<Rightarrow> address = address' \<and> token = token' | _ \<Rightarrow> False) steps"
+\<comment> \<open>Total amount of a given token claimed on the given bridge\<close>
+definition claimedTokenAmount where
+  "claimedTokenAmount address token steps = 
+   sum_list (map CLAIM_amount (tokenClaims address token steps))"
 
-definition claimedAmount where
-  "claimedAmount address token steps = 
-   sum_list (map CLAIM_amount (claims address token steps))"
-
-lemma claimedAmoutConsNonClaim [simp]:
+lemma claimedTokenAmoutConsNonClaim [simp]:
   assumes "\<nexists> address' caller' ID' token' amount' proof'. step = CLAIM address' caller' ID' token' amount' proof'"
-  shows "claimedAmount address token (step # steps) = claimedAmount address token steps"
+  shows "claimedTokenAmount address token (step # steps) = claimedTokenAmount address token steps"
   using assms 
-  unfolding claimedAmount_def claims_def
+  unfolding claimedTokenAmount_def tokenClaims_def
   by (cases step, auto)
-
-definition withdrawals where
-  "withdrawals address token steps = filter (\<lambda> step. case step of WITHDRAW address' caller token' amount proof \<Rightarrow> address = address' \<and> token = token' | _ \<Rightarrow> False) steps"
-
-definition withdrawnAmount where
-  "withdrawnAmount address token steps = 
-   sum_list (map WITHDRAW_amount (withdrawals address token steps))"
-
-lemma withdrawnAmoutConsNonWithdraw [simp]:
-  assumes "\<nexists> address' caller' token' amount' proof'. step = WITHDRAW address' caller' token' amount' proof'"
-  shows "withdrawnAmount address token (step # steps) = withdrawnAmount address token steps"
-  using assms 
-  unfolding withdrawnAmount_def withdrawals_def
-  by (cases step, auto)
-
-definition cancels where
-  "cancels address token steps = 
-   filter (\<lambda> step. case step of CANCEL address' caller ID token' amount proof \<Rightarrow> address = address' \<and> token = token' | _ \<Rightarrow> False) steps"
-
-definition canceledAmount where
-  "canceledAmount address token steps = 
-   sum_list (map CANCEL_amount (cancels address token steps))"
-
-lemma canceledAmountCancel [simp]:
-  shows "canceledAmount address token (CANCEL address caller ID token amount proof # steps) = 
-         amount + canceledAmount address token steps"
-  unfolding canceledAmount_def cancels_def
-  by auto
-
-lemma canceledAmountConsNonCancel [simp]:
-  assumes "\<nexists> address' caller' ID' token' amount' proof'. step = CANCEL address' caller' ID' token' amount' proof'"
-  shows "canceledAmount address token (step # steps) = canceledAmount address token steps"
-  using assms 
-  unfolding canceledAmount_def cancels_def
-  by (cases step, auto)
-
-lemma canceledAmountConsOther [simp]:
-  assumes "address \<noteq> address' \<or> token \<noteq> token'"
-  shows "canceledAmount address token ((CANCEL address' caller' ID' token' amount' proof') # steps) = canceledAmount address token steps"
-  using assms
-  unfolding canceledAmount_def cancels_def
-  by auto
 
 primrec DEPOSIT_id where
   "DEPOSIT_id (DEPOSIT address caller ID token amount) = ID"
 
-definition claimedDeposits where
-  "claimedDeposits tokenDepositAddress bridgeAddress token steps = 
-     filter (\<lambda> step. \<exists> caller' amount' proof'. CLAIM bridgeAddress caller' (DEPOSIT_id step) token amount' proof' \<in> set steps) (deposits tokenDepositAddress token steps)"
+definition isClaimedID where
+ "isClaimedID bridgeAddress token ID steps \<longleftrightarrow> (\<exists> caller' amount' proof'. CLAIM bridgeAddress caller' ID token amount' proof' \<in> set steps)"
 
-definition claimedDepositsAmount where
-  "claimedDepositsAmount tokenDepositAddress bridgeAddress token steps = 
-   sum_list (map DEPOSIT_amount (claimedDeposits tokenDepositAddress bridgeAddress token steps))"
+\<comment> \<open>All deposits of the given token on the given address that have been claimed\<close>
+definition claimedTokenDeposits where
+  "claimedTokenDeposits tokenDepositAddress bridgeAddress token steps = 
+     filter 
+      (\<lambda> step. isClaimedID bridgeAddress token (DEPOSIT_id step) steps) 
+      (tokenDeposits tokenDepositAddress token steps)"
+
+\<comment> \<open>Total amount of tokens that have been deposited on the given address and then claimed\<close>
+definition claimedTokenDepositsAmount where
+  "claimedTokenDepositsAmount tokenDepositAddress bridgeAddress token steps = 
+   sum_list (map DEPOSIT_amount (claimedTokenDeposits tokenDepositAddress bridgeAddress token steps))"
 
 lemma claimedDepositsAmountOther: 
   assumes "\<nexists> caller ID amount. step = DEPOSIT tokenDepositAddress caller ID token amount"
   assumes "\<nexists> caller' ID' amount' proof'. step = CLAIM bridgeAddress caller' ID' token amount' proof'"
-  shows "claimedDepositsAmount tokenDepositAddress bridgeAddress token (step # steps) =
-         claimedDepositsAmount tokenDepositAddress bridgeAddress token steps"
+  shows "claimedTokenDepositsAmount tokenDepositAddress bridgeAddress token (step # steps) =
+         claimedTokenDepositsAmount tokenDepositAddress bridgeAddress token steps"
 proof-
-  have "deposits tokenDepositAddress token (step # steps) = deposits tokenDepositAddress token steps"
+  have "tokenDeposits tokenDepositAddress token (step # steps) = tokenDeposits tokenDepositAddress token steps"
     using assms
-    unfolding deposits_def
+    unfolding tokenDeposits_def
     by (cases step, auto)
-  then have "claimedDeposits tokenDepositAddress bridgeAddress token (step # steps) = 
-             claimedDeposits tokenDepositAddress bridgeAddress token steps"
+  then have "claimedTokenDeposits tokenDepositAddress bridgeAddress token (step # steps) = 
+             claimedTokenDeposits tokenDepositAddress bridgeAddress token steps"
     using assms
-    unfolding claimedDeposits_def
+    unfolding claimedTokenDeposits_def isClaimedID_def
     by (smt (verit, del_insts) filter_cong list.set_intros(2) set_ConsD)
   then show ?thesis
-    unfolding claimedDepositsAmount_def
+    unfolding claimedTokenDepositsAmount_def
     by simp
 qed
 
-lemma filter':
-  assumes "filter P xs = ys1 @ [y] @ ys2" "y \<notin> set (ys1 @ ys2)"
-  assumes "\<forall> x \<in> set xs. P x \<and> x \<noteq> y \<longleftrightarrow> P' x"
-  shows "filter P' xs = ys1 @ ys2"
-  using assms
+end
+
+context InitFirstUpdate
+begin
+
+
+(*
+                   stepsInit                CLAIM
+contractsInit        \<rightarrow>*         contractsI   \<rightarrow>   contractsClaim
+properSetup        UPDATE
+getDeposit=0
+lastState=0
+*)
+
+lemma claimedTokenDepositsAmountsClaim:
+  assumes "reachableFrom contractsI contractsClaim [CLAIM bridgeAddress caller ID token amount proof]"
+  shows   "claimedTokenDepositsAmount tokenDepositAddress bridgeAddress token
+             (CLAIM bridgeAddress caller ID token amount proof # stepsInit) = 
+           claimedTokenDepositsAmount tokenDepositAddress bridgeAddress token stepsInit + amount"
 proof-
-  have "filter (\<lambda>x. x \<noteq> y) ys1 = ys1"
-    using assms(2)
-    by (induction ys1, auto)
-  moreover
-  have "filter (\<lambda>x. x \<noteq> y) ys2 = ys2"
-    using assms(2)
-    by (induction ys2, auto)
-  moreover
-  have "filter P' xs = filter (\<lambda>x. P x \<and> x \<noteq> y) xs"
-  proof (rule filter_cong)
-    fix x
-    assume "x \<in> set xs" then 
-    show "P' x \<longleftrightarrow> P x \<and> x \<noteq> y"
-      using assms
-      by simp
-  qed simp
-  then have "filter P' xs = filter (\<lambda> x. x \<noteq> y) (filter P xs)"
-    by simp
-  ultimately show ?thesis
-    using assms \<open>y \<notin> set (ys1 @ ys2)\<close>
-    by auto
-qed
-
-lemma claimedDepositAmountsClaim [simp]:
-  assumes "properSetup initContracts tokenDepositAddress bridgeAddress"
-  assumes "properToken initContracts tokenDepositAddress bridgeAddress token"
-  assumes "getDeposit (the (tokenDepositState initContracts tokenDepositAddress)) ID = 0"
-  assumes "getLastStateB initContracts bridgeAddress = 0"
-  assumes "let stateOracleAddress = stateOracleAddressB initContracts bridgeAddress
-            in UPDATE stateOracleAddress stateRoot \<in> set steps"
-  assumes "updatesNonZero steps"
-
-  assumes "\<forall> step \<in> set steps. \<forall>caller' amount' ID' token'.
-             step = DEPOSIT tokenDepositAddress caller' ID' token' amount' \<longrightarrow>
-             hash3 caller' token' amount' \<noteq> 0"
-  assumes "hash3 caller token amount \<noteq> 0"
-  assumes "hash3_inj"
-
-  assumes "reachableFrom initContracts contracts' (CLAIM bridgeAddress caller ID token amount proof' # steps)"
-  shows   "claimedDepositsAmount tokenDepositAddress bridgeAddress token
-             (CLAIM bridgeAddress caller ID token amount proof # steps) = 
-           claimedDepositsAmount tokenDepositAddress bridgeAddress token steps + amount"
-proof-  
   define CLAIM_step where 
   "CLAIM_step = CLAIM bridgeAddress caller ID token amount proof"
   define DEPOSIT_step where
   "DEPOSIT_step = DEPOSIT tokenDepositAddress caller ID token amount"
   define claimed where
-  "claimed = claimedDeposits tokenDepositAddress bridgeAddress token (CLAIM_step # steps)"
+  "claimed = claimedTokenDeposits tokenDepositAddress bridgeAddress token (CLAIM_step # stepsInit)"
 
-  have deposits: "deposits tokenDepositAddress token (CLAIM_step # steps) = 
-                  deposits tokenDepositAddress token steps"
+  have deposits: "tokenDeposits tokenDepositAddress token (CLAIM_step # stepsInit) = 
+                  tokenDeposits tokenDepositAddress token stepsInit"
     unfolding CLAIM_step_def
-    by (simp add: local.deposits_def)
+    by (simp add: tokenDeposits_def)
 
-  obtain contracts'' where
-     "reachableFrom initContracts contracts'' steps"
-     "callClaim contracts'' bridgeAddress (message caller amount) ID token amount proof' = (Success, contracts')"
+  have "callClaim contractsI bridgeAddress (message caller amount) ID token amount proof = (Success, contractsClaim)"
     using assms
-    unfolding CLAIM_step_def
-    by (smt (verit) executeStep.simps(2) list.discI list.inject reachableFrom.simps)
-  then have "DEPOSIT_step \<in> set steps"
-    using assms depositBeforeClaim
+    by (metis executeStep.simps(2) reachableFromSingleton)
+  then have "DEPOSIT_step \<in> set stepsInit"
+    using depositBeforeClaim[where msg="message caller amount"]
     unfolding DEPOSIT_step_def
-    by (metis Message.select_convs(1) message_def)
+    by simp
   then have "DEPOSIT_step \<in> set claimed"
     unfolding DEPOSIT_step_def CLAIM_step_def claimed_def
-    unfolding claimedDeposits_def deposits_def
+    unfolding claimedTokenDeposits_def tokenDeposits_def isClaimedID_def
     by auto
 
-  obtain steps1 steps2 where steps: "steps = steps1 @ [DEPOSIT_step] @ steps2"
-    using \<open>DEPOSIT_step \<in> set steps\<close>
+  obtain steps1 steps2 where steps: "stepsInit = steps1 @ [DEPOSIT_step] @ steps2"
+    using \<open>DEPOSIT_step \<in> set stepsInit\<close>
     by (metis Cons_eq_append_conv in_set_conv_decomp self_append_conv2)
 
   have *: "\<forall> step \<in> set (steps1 @ steps2). (\<forall> caller' amount' ID'. step = DEPOSIT tokenDepositAddress caller' ID' token amount' \<longrightarrow> ID' \<noteq> ID)"
-  proof safe
-    fix caller' amount' proof' 
-    assume "DEPOSIT tokenDepositAddress caller' ID token amount' \<in> set (steps1 @ steps2)"
-    moreover
-    have "\<nexists>token' caller' amount'.
-         DEPOSIT tokenDepositAddress caller' ID token' amount' \<in> set (steps1 @ steps2)"
-    proof (rule DEPOSITNoDouble'[OF \<open>reachableFrom initContracts contracts'' steps\<close>])
-      show "steps = steps1 @ [DEPOSIT tokenDepositAddress caller ID token amount] @ steps2"
-        using steps
-        unfolding DEPOSIT_step_def
-        by simp
-    next
-      show "\<forall>step\<in>set steps. \<forall>caller' amount' ID' token'.
-          step = DEPOSIT tokenDepositAddress caller' ID' token' amount' \<longrightarrow>
-          hash3 caller' token' amount' \<noteq> 0"
-        by fact
-    qed
-    ultimately
-    show False
-      by simp
-  qed
+    using DEPOSITNoDouble'[OF reachableFromInitI] steps
+    unfolding DEPOSIT_step_def
+    by auto
   then have "DEPOSIT_step \<notin> set (steps1 @ steps2)"
     unfolding DEPOSIT_step_def
     by auto
 
-  define P' where "P' = (\<lambda> x. ((\<exists>caller' amount' proof'.
-            CLAIM bridgeAddress caller' (DEPOSIT_id x) token amount' proof' \<in> set (CLAIM_step # steps))))"
-  define P where "P = (\<lambda> x. ((\<exists>caller' amount' proof'.
-            CLAIM bridgeAddress caller' (DEPOSIT_id x) token amount' proof' \<in> set steps)))"
-  define Q where "Q = (\<lambda> step. case step of DEPOSIT address' caller ID token' amount \<Rightarrow> tokenDepositAddress = address' \<and> token = token' | _ \<Rightarrow> False)"
+  define P where "P = (\<lambda> step. isClaimedID bridgeAddress token (DEPOSIT_id step) stepsInit)"
+  define P' where "P' = (\<lambda> step. isClaimedID bridgeAddress token (DEPOSIT_id step) (CLAIM_step # stepsInit))"
+  define Q where "Q = (\<lambda> step. isTokenDeposit tokenDepositAddress token step)"
 
-  have "deposits tokenDepositAddress token steps = 
-        (filter Q steps1) @ [DEPOSIT_step] @ (filter Q steps2)"
-    using \<open>steps = steps1 @ [DEPOSIT_step] @ steps2\<close>
-    unfolding deposits_def Q_def DEPOSIT_step_def
+  define depositsInit where "depositsInit = tokenDeposits tokenDepositAddress token stepsInit"
+
+  have "depositsInit = (filter Q steps1) @ [DEPOSIT_step] @ (filter Q steps2)"
+    using \<open>stepsInit = steps1 @ [DEPOSIT_step] @ steps2\<close>
+    unfolding depositsInit_def tokenDeposits_def Q_def DEPOSIT_step_def
     by auto
-  then have **: "claimed = filter P' (filter Q steps1) @ filter P' [DEPOSIT_step] @ filter P' (filter Q steps2)"
+  then have claimed:
+    "claimed = filter P' (filter Q steps1) @ filter P' [DEPOSIT_step] @ filter P' (filter Q steps2)"
     using deposits
-    unfolding claimed_def claimedDeposits_def P'_def
+    unfolding depositsInit_def claimed_def claimedTokenDeposits_def P'_def
     by auto
 
   define c1 where "c1 = filter P' (filter Q steps1)" 
@@ -1456,7 +873,7 @@ proof-
     unfolding c1_def c2_def
     by auto
   then have claimed: "claimed = c1 @ [DEPOSIT_step] @ c2"
-    using ** \<open>DEPOSIT_step \<in> set claimed\<close> 
+    using claimed \<open>DEPOSIT_step \<in> set claimed\<close> 
     unfolding c1_def c2_def
     by (metis append.assoc append.right_neutral filter.simps(1) filter.simps(2))
   
@@ -1466,182 +883,1378 @@ proof-
     unfolding c1_def c2_def
     by auto
 
-  have "filter P (deposits tokenDepositAddress token steps) = c1 @ c2"
+  have "filter P depositsInit = c1 @ c2"
   proof (rule filter')
     show "DEPOSIT_step \<notin> set (c1 @ c2)"
       by fact
   next
-    show "filter P' (deposits tokenDepositAddress token steps) = c1 @ [DEPOSIT_step] @ c2"
+    show "filter P' depositsInit = c1 @ [DEPOSIT_step] @ c2"
       using \<open>claimed = c1 @ [DEPOSIT_step] @ c2\<close> deposits
-      unfolding claimed_def claimedDeposits_def P'_def
+      unfolding depositsInit_def claimed_def claimedTokenDeposits_def P'_def
       by simp
   next
-    show "\<forall> step \<in> set (deposits tokenDepositAddress token steps). (P' step \<and> step \<noteq> DEPOSIT_step) \<longleftrightarrow> P step"
+    show "\<forall> step \<in> set depositsInit. (P' step \<and> step \<noteq> DEPOSIT_step) \<longleftrightarrow> P step"
     proof safe
       fix step
-      assume "step \<in> set (deposits tokenDepositAddress token steps)" "P' step" "step \<noteq> DEPOSIT_step"
+      assume "step \<in> set depositsInit" "P' step" "step \<noteq> DEPOSIT_step"
       have "DEPOSIT_id step \<noteq> ID"
       proof-
         have "step \<in> set (filter Q steps1 @ filter Q steps2)"
-          using \<open>step \<in> set (deposits tokenDepositAddress token steps)\<close> \<open>step \<noteq> DEPOSIT_step\<close>
-          using \<open>deposits tokenDepositAddress token steps = (filter Q steps1) @ [DEPOSIT_step] @ (filter Q steps2)\<close>
+          using \<open>step \<in> set depositsInit\<close> \<open>step \<noteq> DEPOSIT_step\<close>
+          using \<open>depositsInit = (filter Q steps1) @ [DEPOSIT_step] @ (filter Q steps2)\<close>
           by auto
         then have "step \<in> set (steps1 @ steps2)" "Q step"
           by auto
         then obtain ID' caller' amount' where "step = DEPOSIT tokenDepositAddress caller' ID' token amount'"
           unfolding Q_def
-          by (cases step, auto split: Step.splits)
+          by (metis isTokenDeposit.elims(2))
         then show ?thesis
           using * \<open>step \<in> set (steps1 @ steps2)\<close>
           by simp
       qed
       then show "P step"
         using \<open>P' step\<close>
-        unfolding P_def P'_def CLAIM_step_def
+        unfolding P_def P'_def CLAIM_step_def isClaimedID_def
         by auto
     next
-      fix x
-      assume "x \<in> set (deposits tokenDepositAddress token steps)" "P x"
-      then show "P' x"
-        unfolding P_def P'_def
+      fix step
+      assume "step \<in> set depositsInit" "P step"
+      then show "P' step"
+        unfolding P_def P'_def isClaimedID_def
         by auto
     next
-      fix x
       assume "P DEPOSIT_step"
+      have "reachableFrom contractsInit contractsClaim (CLAIM bridgeAddress caller ID token amount proof # stepsInit)"
+        by (meson assms(1) reachableFromInitI reachableFromSingleton reachableFrom_step)
       then show False
-        unfolding P_def DEPOSIT_step_def
-        using CLAIMNoDoubleCons[OF assms(10)]
+        using CLAIMNoDoubleCons \<open>P DEPOSIT_step\<close>
+        unfolding P_def DEPOSIT_step_def isClaimedID_def depositsInit_def
         by auto
     qed
   qed
-  then have "claimedDeposits tokenDepositAddress bridgeAddress token steps = c1 @ c2"
-    unfolding claimed_def P_def claimedDeposits_def
+  then have "claimedTokenDeposits tokenDepositAddress bridgeAddress token stepsInit = c1 @ c2"
+    unfolding claimed_def P_def claimedTokenDeposits_def depositsInit_def
     by auto
   ultimately
   show ?thesis
-    unfolding claimed_def claimedDepositsAmount_def
-    unfolding CLAIM_step_def DEPOSIT_step_def
+    unfolding claimed_def claimedTokenDepositsAmount_def
+    unfolding CLAIM_step_def DEPOSIT_step_def depositsInit_def
     by simp
 qed
 
-lemma claimedDepositAmountsClaimOtherAddress [simp]:
-  assumes "address \<noteq> bridgeAddress"
-  shows "claimedDepositsAmount tokenDepositAddress bridgeAddress token
-          (CLAIM address caller ID token amount proof' # steps) = 
-         claimedDepositsAmount tokenDepositAddress bridgeAddress token steps"
-  using assms
-  by (simp add: claimedDepositsAmountOther)
+(*
+                steps               DEPOSIT
+contractsInit    \<rightarrow>*     contractsI    \<rightarrow>   contractsDeposit
+properSetup
+getDeposit=0
+lastState=0
+*)
+lemma claimedTokenDepositsAmountDeposit:
+  assumes "reachableFrom contractsI contractsDeposit [DEPOSIT tokenDepositAddress caller ID token amount]"
+  shows "claimedTokenDepositsAmount tokenDepositAddress bridgeAddress token
+            (DEPOSIT tokenDepositAddress caller ID token amount # stepsInit) =
+         claimedTokenDepositsAmount tokenDepositAddress bridgeAddress token stepsInit"
+proof-
+  define DEPOSIT_step where "DEPOSIT_step = DEPOSIT tokenDepositAddress caller ID token amount"
+  have "claimedTokenDeposits tokenDepositAddress bridgeAddress token (DEPOSIT_step # stepsInit) = 
+        claimedTokenDeposits tokenDepositAddress bridgeAddress token stepsInit"
+  proof-
+    have "tokenDeposits tokenDepositAddress token (DEPOSIT_step # stepsInit) = 
+          DEPOSIT_step # tokenDeposits tokenDepositAddress token stepsInit"
+      unfolding tokenDeposits_def DEPOSIT_step_def
+      by simp
 
-lemma
-  assumes "reachableFrom initContracts contracts steps"
-  assumes "properSetup initContracts tokenDepositAddress bridgeAddress"
-  assumes "properToken initContracts tokenDepositAddress bridgeAddress token"
-  assumes "bridgeMintedToken contracts bridgeAddress token = mintedToken"
-  assumes "mintedToken \<noteq> token"
-  assumes "\<not> (bridgeDead contracts tokenDepositAddress)"
-  shows "totalBalance (the (ERC20state contracts mintedToken)) = 
-         totalBalance (the (ERC20state initContracts mintedToken)) + claimedDepositsAmount tokenDepositAddress bridgeAddress token steps"
-  using assms
-proof (induction initContracts contracts steps rule: reachableFrom.induct)
-  case (reachableFrom_base initContracts)
-  then show ?case
-    by (simp add: claimedDepositsAmount_def claimedDeposits_def)
-next
-  case (reachableFrom_step steps contracts' initContracts contracts blockNum block step)
-  then have *: "reachableFrom initContracts contracts' (step # steps)"
-    using reachableFrom.reachableFrom_step by blast
-  have notDead: "\<not> bridgeDead contracts tokenDepositAddress"
-    by (metis reachableFrom.simps reachableFromDeadState reachableFrom_step.hyps(2) reachableFrom_step.prems(5))
-  show ?case
-  proof (cases step)
-    case (DEPOSIT address' caller ID token' amount)
-    show ?thesis
-    proof (cases "address' = tokenDepositAddress \<and> token = token'")
-      case False
-      have "token' \<noteq> mintedToken"
-        sorry (* no direct deposit on minted token *)
-      then have "ERC20state contracts' mintedToken = ERC20state contracts mintedToken"
-        using DEPOSIT reachableFrom_step.prems reachableFrom_step.hyps callDepositOtherToken
-        by (metis executeStep.simps(1))
-      moreover 
-      have "claimedDepositsAmount tokenDepositAddress bridgeAddress token steps =
-            claimedDepositsAmount tokenDepositAddress bridgeAddress token (DEPOSIT address' caller ID token' amount # steps)"
-        using claimedDepositsAmountOther False
-        using False
+    moreover
+
+    have reach: "reachableFrom contractsInit contractsDeposit (DEPOSIT_step # stepsInit)"
+      by (metis DEPOSIT_step_def assms reachableFromInitI reachableFromSingleton reachableFrom_step)
+
+    have "\<nexists> caller' amount' proof'. CLAIM bridgeAddress caller' ID token amount' proof' \<in> set stepsInit"
+    proof (rule ccontr)
+      assume "\<not> ?thesis"
+      then obtain caller' amount' proof' where CLAIM_in_steps: "CLAIM bridgeAddress caller' ID token amount' proof' \<in> set stepsInit"
         by auto
-      ultimately show ?thesis
-        using * notDead reachableFrom_step DEPOSIT
+      define CLAIM_step where "CLAIM_step = CLAIM bridgeAddress caller' ID token amount' proof'"
+      have CLAIM_in_steps: "CLAIM_step \<in> set (DEPOSIT_step # stepsInit)"
+        using CLAIM_in_steps
+        unfolding CLAIM_step_def
         by simp
-    next
-      case True
-      have "claimedDepositsAmount tokenDepositAddress bridgeAddress token (step # steps) = 
-            claimedDepositsAmount tokenDepositAddress bridgeAddress token steps"
-        sorry
-      then show ?thesis
-        using True * notDead reachableFrom_step DEPOSIT
-        by simp
-    qed
-  next
-    case (CLAIM address' caller ID token' amount proof')
-    show ?thesis
-    proof (cases "address' = bridgeAddress \<and> token' = token")
-      case True
-      have "totalBalance (the (ERC20state contracts' mintedToken))  = 
-            totalBalance (the (ERC20state contracts mintedToken)) + amount"
-      proof (rule callClaimTotalBalance)
-        show "finite (Mapping.keys (balances (the (ERC20state contracts mintedToken))))"
-          sorry
+      obtain steps1 steps2 c1 c2 blockNum block where *:
+        "reachableFrom contractsInit c1 steps2"
+        "executeStep c1 blockNum block CLAIM_step = (Success, c2)"
+        "reachableFrom c2 contractsDeposit steps1"
+        "DEPOSIT_step # stepsInit = steps1 @ [CLAIM_step] @ steps2"
+        using reachableFromStepInSteps[OF reach CLAIM_in_steps]
+        unfolding DEPOSIT_step_def
+        by metis
+
+      define DEPOSIT_step' where "DEPOSIT_step' = DEPOSIT tokenDepositAddress (sender (message caller' amount')) ID token amount'"
+
+      interpret Init': Init
+        by unfold_locales
+
+      interpret InitFirstUpdate': InitFirstUpdate where contractsI=c1 and stepsInit=steps2
+      proof
+        show "reachableFrom contractsInit c1 steps2" by fact
       next
-        show "callClaim contracts bridgeAddress (message caller amount) ID token' amount proof' = (Success, contracts')"
-          using True CLAIM reachableFrom_step
+        show "updatesNonZero steps2"
+          by (metis "*"(4) Cons_eq_append_conv add_cancel_right_right list.size(4) nat.simps(3) updatesNonZeroAppend(2) updatesNonZeroInit)
+      next
+        show "steps2 \<noteq> [] \<and> last steps2 = UPDATE (stateOracleAddressB contractsInit bridgeAddress) stateRootInit"
+          by (metis "*"(4) CLAIM_step_def Nil_is_append_conv Step.distinct(10) firstUpdate last.simps last_append not_Cons_self)
+      qed
+
+      have "DEPOSIT_step' \<in> set steps2"
+       using * InitFirstUpdate'.depositBeforeClaim
+       unfolding CLAIM_step_def DEPOSIT_step'_def
+       by fastforce
+
+      moreover
+      obtain steps1' where "steps1 = DEPOSIT_step # steps1'"
+        using *(4)
+        unfolding DEPOSIT_step_def CLAIM_step_def
+        by (metis Cons_eq_append_conv Step.simps(6) list.sel(1))
+      ultimately
+      have "DEPOSIT_step' \<in> set stepsInit"
+        using *(4)
+        by auto
+      then obtain d1 d2 where "DEPOSIT_step # stepsInit = [] @ [DEPOSIT_step] @ d1 @ [DEPOSIT_step'] @ d2"
+        by (metis append.left_neutral append_Cons split_list_first)
+      then show False
+        using DEPOSITNoDouble reach
+        unfolding DEPOSIT_step_def DEPOSIT_step'_def
+        by blast
+    qed
+    ultimately show ?thesis
+      unfolding claimedTokenDeposits_def
+      using DEPOSIT_id.simps DEPOSIT_step_def isClaimedID_def
+      by auto
+  qed
+  then show ?thesis
+    unfolding claimedTokenDepositsAmount_def DEPOSIT_step_def
+    by simp
+qed
+
+end
+
+context HashProofVerifier
+begin
+
+lemma InitInduction [simp]:
+assumes "Init hash2 hash3 generateStateRoot verifyDepositProof generateDepositProof verifyClaimProof generateClaimProof
+         verifyBalanceProof generateBalanceProof tokenDepositAddress bridgeAddress contractsInit contractsI
+         (step # steps)"
+assumes "reachableFrom contractsInit contractsI' steps"
+assumes "executeStep contractsI' blockNum block step = (Success, contractsI)"
+shows "Init hash2 hash3 generateStateRoot verifyDepositProof generateDepositProof verifyClaimProof generateClaimProof
+       verifyBalanceProof generateBalanceProof tokenDepositAddress bridgeAddress contractsInit contractsI' steps"
+  using assms
+  by (simp add: Init_def Init_axioms_def)
+
+lemma InitFirstAxiomsInduction [simp]:
+  assumes "InitFirstUpdate hash2 hash3 generateStateRoot verifyDepositProof generateDepositProof verifyClaimProof
+     generateClaimProof verifyBalanceProof generateBalanceProof tokenDepositAddress bridgeAddress contractsInit
+     contractsI (step # steps) stateRootInit"
+  assumes "reachableFrom contractsInit contractsI' steps"
+  assumes "executeStep contractsI' blockNum block step = (Success, contractsI)"
+  assumes "steps \<noteq> []"
+  shows "InitFirstUpdate hash2 hash3 generateStateRoot verifyDepositProof generateDepositProof verifyClaimProof
+      generateClaimProof verifyBalanceProof generateBalanceProof tokenDepositAddress bridgeAddress contractsInit
+      contractsI' steps stateRootInit"
+  using assms
+  unfolding InitFirstUpdate_def InitFirstUpdate_axioms_def
+  by (metis InitInduction last_ConsR updatesNonZeroCons(1))
+end
+
+context InitFirstUpdate
+begin
+
+(*               [steps]
+   contractsInit   \<rightarrow>*    contracts 
+                           \<not> dead
+*)
+lemma totalBalanceMintedTokenBridgeNotDead:
+  assumes "properToken contractsInit tokenDepositAddress bridgeAddress token"
+  assumes "bridgeMintedToken contractsInit bridgeAddress token = mintedToken"
+  assumes "mintedToken \<noteq> token"
+  assumes "\<not> bridgeDead contractsI tokenDepositAddress"
+  shows "totalBalance (the (ERC20state contractsI mintedToken)) = 
+         totalBalance (the (ERC20state contractsInit mintedToken)) + claimedTokenDepositsAmount tokenDepositAddress bridgeAddress token stepsInit"
+  using reachableFromInitI assms InitFirstUpdate_axioms
+proof (induction contractsInit contractsI stepsInit rule: reachableFrom.induct)
+  case (reachableFrom_base contractsInit)
+  then show ?case
+    by (simp add: claimedTokenDepositsAmount_def claimedTokenDeposits_def isClaimedID_def)
+next
+  case (reachableFrom_step steps contractsI contractsInit contractsI' blockNum block step)
+
+  show ?case
+  proof (cases "steps = []")
+    case True
+    then have "reachableFrom contractsInit contractsI' []"
+      using reachableFrom_step.hyps
+      by simp
+    then have "contractsInit = contractsI'"
+      using reachableFrom.cases
+      by blast
+    then have "totalBalance (the (ERC20state contractsI' mintedToken)) =
+        totalBalance (the (ERC20state contractsInit mintedToken))"
+      by simp
+    moreover
+    have "claimedTokenDepositsAmount tokenDepositAddress bridgeAddress token
+          [UPDATE (stateOracleAddressB contractsInit bridgeAddress) stateRootInit] = 0"
+      by (simp add: claimedTokenDepositsAmount_def claimedTokenDeposits_def tokenDeposits_def)
+    moreover
+    have "step = UPDATE (stateOracleAddressB contractsInit bridgeAddress) stateRootInit"
+      by (metis InitFirstUpdate.firstUpdate True last.simps reachableFrom_step.prems(5))
+    ultimately
+    show ?thesis
+      using reachableFrom_step.prems reachableFrom_step.hyps firstUpdate True
+      by simp
+  next
+    case False
+
+    interpret InitFirstUpdate': InitFirstUpdate  where contractsInit=contractsInit and contractsI=contractsI' and stepsInit=steps
+      using False InitFirstAxiomsInduction reachableFrom_step.hyps(1) reachableFrom_step.hyps(2) reachableFrom_step.prems(5) by blast
+
+    have *: "reachableFrom contractsInit contractsI (step # steps)"
+      using reachableFrom.reachableFrom_step reachableFrom_step
+      by blast
+    have notDead: "\<not> bridgeDead contractsI' tokenDepositAddress"
+      using False
+      using reachableFrom.reachableFrom_step reachableFromBridgeDead reachableFrom_base reachableFrom_step.hyps(2) reachableFrom_step.prems(4)
+      by blast
+
+    have *: "totalBalance (the (ERC20state contractsI' mintedToken)) =
+             totalBalance (the (ERC20state contractsInit mintedToken)) +
+             claimedTokenDepositsAmount tokenDepositAddress bridgeAddress token steps"
+      using reachableFrom_step.IH reachableFrom_step.prems
+      using InitFirstUpdate'.InitFirstUpdate_axioms notDead 
+      by fastforce
+
+    show ?thesis
+    proof (cases step)
+      case (DEPOSIT address' caller ID token' amount)
+      show ?thesis
+      proof (cases "address' = tokenDepositAddress \<and> token' = token")
+        case False
+        have "token' \<noteq> mintedToken"
+          sorry (* no direct deposit on minted token *)
+        then have "ERC20state contractsI mintedToken = ERC20state contractsI' mintedToken"
+          using DEPOSIT reachableFrom_step.prems reachableFrom_step.hyps callDepositOtherToken
+          by (metis executeStep.simps(1))
+        moreover 
+        have "claimedTokenDepositsAmount tokenDepositAddress bridgeAddress token steps =
+              claimedTokenDepositsAmount tokenDepositAddress bridgeAddress token (DEPOSIT address' caller ID token' amount # steps)"
+          using claimedDepositsAmountOther False
+          using False
+          by auto
+        ultimately show ?thesis
+          using * reachableFrom_step.prems DEPOSIT
           by simp
       next
-        show "bridgeMintedToken contracts bridgeAddress token' = mintedToken"
-          by (metis ProofVerifier.reachableFromBridgeMintedToken ProofVerifier.reachableFrom_step ProofVerifier_axioms True reachableFrom_step.hyps(1) reachableFrom_step.hyps(2) reachableFrom_step.prems(3))
+        case True
+        have "claimedTokenDepositsAmount tokenDepositAddress bridgeAddress token (step # steps) = 
+              claimedTokenDepositsAmount tokenDepositAddress bridgeAddress token steps"
+          using InitFirstUpdate'.claimedTokenDepositsAmountDeposit
+          using DEPOSIT True reachableFrom.reachableFrom_step reachableFrom_base reachableFrom_step.hyps(2) 
+          by blast
+        then show ?thesis
+          using * 
+          using DEPOSIT True callDepositOtherToken executeStep.simps(1) reachableFrom_step.hyps(2) reachableFrom_step.prems(3)
+          by metis
       qed
-      then show ?thesis
-        using True CLAIM reachableFrom_step * notDead
-        sorry
     next
-      case False
-      have "mintedToken \<noteq> bridgeMintedToken initContracts address' token'" (* no cancel of minted tokens *)
-        sorry
-      then have "ERC20state contracts' mintedToken = ERC20state contracts mintedToken"
-        using CLAIM reachableFrom_step callClaimOtherToken[of contracts address' "message caller amount" ID token' amount proof' contracts' _ mintedToken]
-        by auto
+      case (CLAIM address' caller ID token' amount proof')
+      show ?thesis
+      proof (cases "address' = bridgeAddress \<and> token' = token")
+        case True
+        have "totalBalance (the (ERC20state contractsI mintedToken))  = 
+              totalBalance (the (ERC20state contractsI' mintedToken)) + amount"
+        proof (rule callClaimTotalBalance)
+          show "finite (Mapping.keys (balances (the (ERC20state contractsI' mintedToken))))"
+            sorry
+        next
+          show "callClaim contractsI' bridgeAddress (message caller amount) ID token' amount proof' = (Success, contractsI)"
+            using True CLAIM reachableFrom_step.hyps
+            by simp
+        next
+          show "bridgeMintedToken contractsI' bridgeAddress token' = mintedToken"
+            using True reachableFromBridgeMintedToken reachableFrom_step.hyps(1) reachableFrom_step.prems(2) 
+            by blast
+        qed
+
+        moreover
+
+        have "claimedTokenDepositsAmount tokenDepositAddress bridgeAddress token
+                  (CLAIM bridgeAddress caller ID token amount proof' # steps) =
+              claimedTokenDepositsAmount tokenDepositAddress bridgeAddress token steps + amount"
+        proof (rule InitFirstUpdate'.claimedTokenDepositsAmountsClaim)
+          show "reachableFrom contractsI' contractsI [CLAIM bridgeAddress caller ID token amount proof']"
+            using CLAIM True reachableFrom.reachableFrom_step reachableFrom_base reachableFrom_step.hyps(2) by blast
+        qed
+
+        ultimately
+        
+        show ?thesis
+          using * CLAIM True
+          by simp
+      next
+        case False
+        have "mintedToken \<noteq> bridgeMintedToken contractsInit address' token'" (* no cancel of minted tokens *)
+          sorry
+        then have "ERC20state contractsI mintedToken = ERC20state contractsI' mintedToken"
+          using CLAIM callClaimOtherToken[where msg="message caller amount"]
+          by (metis executeStep.simps(2) reachableFromBridgeMintedToken InitFirstUpdate'.reachableFromInitI reachableFrom_step.hyps(2))
+        then show ?thesis
+          using False CLAIM reachableFrom_step *
+          by (auto simp add: claimedDepositsAmountOther)
+      qed
+    next
+      case (UPDATE address' stateRoot')
       then show ?thesis
-        using False CLAIM reachableFrom_step * notDead
-        by (auto simp add: claimedDepositsAmountOther)
+        using reachableFrom_step *
+        using claimedDepositsAmountOther
+        by simp
+    next
+      case (CANCEL address' caller' ID' token' amount' proof')
+      have "mintedToken \<noteq> token'" (* no cancel of minted tokens *)
+        sorry
+      then have "ERC20state contractsI mintedToken = ERC20state contractsI' mintedToken"
+        using CANCEL reachableFrom_step.hyps(2) by auto
+      then show ?thesis
+        using CANCEL reachableFrom_step *
+        using claimedDepositsAmountOther
+        by simp
+    next
+      case (WITHDRAW address' caller token' amount proof')
+      have "mintedToken \<noteq> token'" (* no withdrawal of minted tokens *)
+        sorry
+      then have "ERC20state contractsI mintedToken = ERC20state contractsI' mintedToken"
+        using WITHDRAW reachableFrom_step.hyps(2) by auto
+      moreover
+      have "claimedTokenDepositsAmount tokenDepositAddress bridgeAddress token (step # steps) = 
+            claimedTokenDepositsAmount tokenDepositAddress bridgeAddress token steps"
+        using claimedDepositsAmountOther WITHDRAW
+        by simp
+      ultimately
+      show ?thesis
+        using WITHDRAW reachableFrom_step *
+        by simp
     qed
-  next
-    case (UPDATE address' stateRoot')
-    then show ?thesis
-      using reachableFrom_step *
-      using claimedDepositsAmountOther
-      by simp
-  next
-    case (CANCEL address' caller' ID' token' amount' proof')
-    have "mintedToken \<noteq> token'" (* no cancel of minted tokens *)
-      sorry
-    then have "ERC20state contracts' mintedToken = ERC20state contracts mintedToken"
-      using CANCEL reachableFrom_step.hyps(2) by auto
-    then show ?thesis
-      using CANCEL reachableFrom_step * notDead
-      using claimedDepositsAmountOther
-      by simp
-  next
-    case (WITHDRAW address' caller token' amount proof')
-    have "mintedToken \<noteq> token'" (* no withdrawal of minted tokens *)
-      sorry
-   then have "ERC20state contracts' mintedToken = ERC20state contracts mintedToken"
-      using WITHDRAW reachableFrom_step.hyps(2) by auto
-    then show ?thesis
-      using WITHDRAW reachableFrom_step * notDead
-      using claimedDepositsAmountOther
-      by simp
   qed
 qed
 
 end
 
+context HashProofVerifier
+begin
+
+lemma
+  assumes "reachableFrom contractsInit contracts steps"
+  assumes "\<not> bridgeDead contracts tokenDepositAddress"
+  shows "balanceOf (the (ERC20state contracts token)) tokenDepositAddress = 
+         balanceOf (the (ERC20state contractsInit token)) tokenDepositAddress + depositedTokenAmount tokenDepositAddress token steps"
+  using assms
+proof (induction contractsInit contracts steps rule: reachableFrom.induct)
+  case (reachableFrom_base contractsInit)
+  then show ?case
+    by (simp add: depositedTokenAmount_def tokenDeposits_def)
+next
+  case (reachableFrom_step steps contracts' contractsInit contracts blockNum block step)
+  have notDead: "\<not> bridgeDead contracts tokenDepositAddress"
+    by (meson reachableFrom.intros(1) reachableFrom.reachableFrom_step reachableFromBridgeDead reachableFrom_step.hyps(2) reachableFrom_step.prems)
+
+  then have *: 
+    "balanceOf (the (ERC20state contracts token)) tokenDepositAddress =
+     balanceOf (the (ERC20state contractsInit token)) tokenDepositAddress +
+     depositedTokenAmount tokenDepositAddress token steps"
+    using reachableFrom_step.IH
+    by simp
+
+  show ?case
+  proof (cases step)
+    case (DEPOSIT address' caller ID token' amount)
+    have "caller \<noteq> tokenDepositAddress"
+      sorry
+    show ?thesis
+    proof (cases "address' = tokenDepositAddress \<and> token' = token")
+      case False
+      then show ?thesis
+        using reachableFrom_step DEPOSIT \<open>caller \<noteq> tokenDepositAddress\<close>
+        using callDepositBalanceOfOther notDead callDepositOtherToken depositedTokenAmountConsOther 
+        by (metis executeStep.simps(1) senderMessage)
+    next
+      case True
+      then show ?thesis
+        using reachableFrom_step DEPOSIT
+        using callDepositBalanceOfContract notDead
+        by auto
+    qed
+  next
+    case (CLAIM address' caller ID token' amount proof')
+    have "bridgeMintedToken contractsInit address' token' \<noteq> token"
+      sorry (* no tokens are minted on the token contract *)
+    then show ?thesis
+      using * reachableFrom_step.hyps CLAIM
+      using callClaimOtherToken
+      by auto
+  next
+    case (UPDATE address' stateRoot')
+    then show ?thesis
+      using * reachableFrom_step.hyps
+      by simp
+  next
+    case (WITHDRAW address' caller token' amount proof')
+    show ?thesis
+    proof (cases "address' = tokenDepositAddress")
+      case True
+      then show ?thesis
+        using WITHDRAW * reachableFrom_step.hyps reachableFrom_step.prems
+        by (simp add: callWithdrawWhileDeadBridgeDead)
+    next
+      case False
+      show ?thesis
+      proof (cases "token = token'")
+        case True
+        have "caller \<noteq> tokenDepositAddress"
+          sorry
+        then have "balanceOf (the (ERC20state contracts' token)) tokenDepositAddress =
+                   balanceOf (the (ERC20state contracts token)) tokenDepositAddress"
+          using WITHDRAW reachableFrom_step notDead
+          using True False callWithdrawWhileDead_balanceOfOther[of contracts address' "message caller 0"]
+          by auto
+        then show ?thesis
+          using False WITHDRAW reachableFrom_step notDead
+          by auto
+      next
+        case False
+        then show ?thesis
+          using WITHDRAW reachableFrom_step.hyps *
+          by (metis Step.simps(12) callWithdrawWhileDeadOtherToken depositedTokenAmoutConsNonDeposit executeStep.simps(5))
+      qed
+    qed
+  next
+    case (CANCEL address' caller' ID' token' amount' proof')
+    show ?thesis
+    proof (cases "address' = tokenDepositAddress")
+      case True
+      then have "bridgeDead contracts' tokenDepositAddress"
+        using CANCEL reachableFrom_step
+        using callCancelDepositWhileDeadBridgeDead 
+        by (metis executeStep.simps(4))
+      then show ?thesis
+        using reachableFrom_step
+        by blast
+    next
+      case False
+      have "caller' \<noteq> tokenDepositAddress"
+        sorry
+      then show ?thesis
+        using callCancelDepositWhileDead_balanceOfOther callCancelDepositOtherToken 
+        using False CANCEL reachableFrom_step notDead
+        by (metis Message.select_convs(1) Step.simps(10) depositedTokenAmoutConsNonDeposit executeStep.simps(4) message_def)
+    qed
+  qed
+qed
+
+end
+
+(* ------------------------------------------------------------------------------------ *)
+context HashProofVerifier
+begin
+
+text \<open>No deposit after the bridge dies\<close>
+theorem noDepositBridgeDead: 
+  assumes "bridgeDead contracts tokenDepositAddress"
+  assumes "reachableFrom contracts contracts' steps"
+  shows "fst (callDeposit contracts' tokenDepositAddress block msg ID token amount) \<noteq> Success"
+  using assms callDepositFailsInDeadState reachableFromBridgeDead
+  by blast
+
+end
+
+(*
+               [stepsInit]                  update                  [stepsNoUpdate]               stepDeath               stepsBD
+   contractsInit  \<rightarrow>*   contractsLastUpdate'  \<rightarrow>  contractsLastUpdate       \<rightarrow>*     contractsDead'     \<rightarrow>    contractsDead   \<rightarrow>*  contractsBD
+   properSetup
+*)
+locale BridgeDead = StrongHashProofVerifier +
+  fixes contractsInit :: Contracts
+  fixes contractsLastUpdate' :: Contracts
+  fixes contractsLastUpdate  :: Contracts
+  fixes contractsDead' :: Contracts
+  fixes contractsDead :: Contracts
+  fixes contractsBD :: Contracts
+  fixes tokenDepositAddress :: address
+  fixes bridgeAddress :: address
+  fixes stepsInit :: "Step list"
+  fixes stepsNoUpdate :: "Step list"
+  fixes stepsBD :: "Step list"
+  fixes stepDeath :: Step
+  fixes stateRoot :: bytes32
+  fixes blockLU :: Block
+  fixes blockNumLU :: uint256
+
+  assumes properSetupInit [simp]:
+    "properSetup contractsInit tokenDepositAddress bridgeAddress"
+  assumes reachableFromInitLastUpdate' [simp]: 
+    "reachableFrom contractsInit contractsLastUpdate' stepsInit"
+  \<comment> \<open>The last update that happened when the bridge was still alive\<close>
+  assumes lastUpdate [simp]:
+    "let stateOracleAddress = stateOracleAddressB contractsInit bridgeAddress
+      in callUpdate contractsLastUpdate' stateOracleAddress blockLU blockNumLU stateRoot = (Success, contractsLastUpdate)"
+  \<comment> \<open>There were no updates since then until the bridge died\<close>
+  assumes reachableFromLastUpdateDead [simp]: 
+    "reachableFrom contractsLastUpdate contractsDead' stepsNoUpdate"
+  assumes noUpdatesLastUpdateDead [simp]:
+    "let stateOracleAddress = stateOracleAddressB contractsInit bridgeAddress
+      in \<nexists> stateRoot'. UPDATE stateOracleAddress stateRoot' \<in> set stepsNoUpdate"
+  \<comment> \<open>Bridge died\<close>
+  assumes notBridgeDead' [simp]:
+    "\<not> bridgeDead contractsDead' tokenDepositAddress"
+  assumes deathStep [simp]: 
+    "reachableFrom contractsDead' contractsDead [stepDeath]"
+  assumes bridgeDead [simp]:
+    "bridgeDead contractsDead tokenDepositAddress"
+  \<comment> \<open>Current contracts are reached\<close>
+  assumes reachableFromContractsBD [simp]:
+    "reachableFrom contractsDead contractsBD stepsBD"
+
+  (* NOTE: additional assumptions *)
+  assumes stateRootNonZero:
+    "stateRoot \<noteq> 0"
+begin
+lemma properSetupLastUpdate' [simp]:
+  shows "properSetup contractsLastUpdate' tokenDepositAddress bridgeAddress"
+  using properSetupReachable properSetupInit reachableFromInitLastUpdate'
+  by blast
+
+lemma stateOracleAddressBLastUpdate' [simp]:
+  shows "stateOracleAddressB contractsLastUpdate' bridgeAddress =
+         stateOracleAddressB contractsInit bridgeAddress"
+  using reachableFromBridgeStateOracle reachableFromInitLastUpdate' 
+  by blast
+
+lemma stateOracleAddressBLastUpdate [simp]:
+  shows "stateOracleAddressB contractsLastUpdate bridgeAddress =
+         stateOracleAddressB contractsInit bridgeAddress"
+  using callUpdateIBridge lastUpdate stateOracleAddressBLastUpdate' 
+  by presburger
+end
+
+sublocale BridgeDead \<subseteq> LastUpdate
+  where contractsLU=contractsDead'
+proof
+  show "let stateOracleAddress = stateOracleAddressB contractsLastUpdate bridgeAddress
+         in \<nexists>stateRoot'. UPDATE stateOracleAddress stateRoot' \<in> set stepsNoUpdate"
+    using noUpdatesLastUpdateDead
+    by simp
+next
+qed simp_all
+
+context BridgeDead
+begin
+
+lemma reachableFromInitDead' [simp]: 
+  shows "reachableFrom contractsInit contractsDead' (stepsNoUpdate @ [UPDATE_step] @ stepsInit)"
+  using reachableFromInitLastUpdate' reachableFromLastUpdate'LastUpdate reachableFromLastUpdateDead reachableFromTrans
+  by presburger
+
+lemma reachableFromInitBD [simp]: 
+  shows "reachableFrom contractsInit contractsBD (stepsBD @ [stepDeath] @ stepsNoUpdate @ [UPDATE_step] @ stepsInit)"
+  using reachableFromContractsBD deathStep reachableFromInitDead' reachableFromTrans
+  by blast
+
+lemma properSetupDead [simp]:
+  shows "properSetup contractsDead tokenDepositAddress bridgeAddress"
+  using properSetupReachable deathStep properSetupLU 
+  by blast
+
+lemma properSetupBD [simp]:
+  shows "properSetup contractsBD tokenDepositAddress bridgeAddress"
+  using reachableFromContractsBD properSetupDead properSetupReachable 
+  by blast
+
+
+lemma tokenDepositStateContractsCurrentNotNone [simp]:
+  shows "tokenDepositState contractsBD tokenDepositAddress \<noteq> None"
+  by (meson properSetupBD properSetup_def)
+
+lemma ERC20stateLastUpdate' [simp]:
+  assumes "properToken contractsInit tokenDepositAddress bridgeAddress token"
+  shows "ERC20state contractsLastUpdate' token \<noteq> None"
+  using properTokenReachable[OF reachableFromInitLastUpdate' assms(1)]
+  by (meson properToken_def)
+
+lemma ERC20stateContractsCurrentNotNone [simp]:
+  assumes "properToken contractsInit tokenDepositAddress bridgeAddress token"
+  shows "ERC20state contractsBD token \<noteq> None"
+  using assms
+  by (meson reachableFromERC20State properToken_def reachableFromInitBD)
+
+lemma notBridgeDeadContractsLastUpdate':
+  shows "\<not> bridgeDead contractsLastUpdate' tokenDepositAddress"
+proof-
+  have "reachableFrom contractsLastUpdate' contractsDead' (stepsNoUpdate @ [UPDATE_step])"
+    using reachableFromLastUpdate'LastUpdate reachableFromLastUpdateDead reachableFromTrans
+    by blast
+  then show ?thesis
+    using notBridgeDead' reachableFromBridgeDead
+    by blast
+qed
+
+lemma bridgeDeadContractsBD [simp]:
+  shows "bridgeDead contractsBD tokenDepositAddress"
+  using reachableFromBridgeDead bridgeDead reachableFromContractsBD
+  by blast
+
+lemma getLastStateBLastUpdate [simp]:
+  shows "getLastStateB contractsLastUpdate bridgeAddress = stateRoot"
+  using callUpdateLastState lastUpdate stateOracleAddressBLastUpdate
+  by presburger
+
+lemmas properSetupDead' = properSetupLU
+lemmas getLastStateBDead' = getLastStateBLU
+lemmas getLastStateTDDead' = getLastStateTDLU
+
+lemma stepDeathNoUpdate [simp]:
+  shows "\<nexists> address stateRoot. stepDeath = UPDATE address stateRoot"
+  using bridgeDead callUpdateDeadState deathStep notBridgeDead'
+  by (smt (verit) executeStep.simps(3) list.distinct(1) reachableFrom.simps reachableFromCons')
+
+lemma deadStateContractsDead [simp]: 
+  shows "deadState (the (tokenDepositState contractsDead tokenDepositAddress)) = stateRoot"
+  using BridgeDiesDeadState bridgeDead deathStep getLastStateTDLU notBridgeDead'  
+  by (smt (verit) list.discI reachableFrom.simps reachableFromCons')
+
+lemma deadStateContractsBD [simp]: 
+  shows "deadState (the (tokenDepositState contractsBD tokenDepositAddress)) = stateRoot"
+  using stateRootNonZero reachableFromContractsBD deadStateContractsDead reachableFromDeadState
+  by blast
+
+theorem cancelDepositWhileDeadNoClaim:
+  \<comment> \<open>Cancel deposit succeded\<close>
+  assumes cancel:
+     "callCancelDepositWhileDead contractsBD tokenDepositAddress msg block ID token amount proof = 
+      (Success, contractsCancel)"
+  \<comment> \<open>Claim did not happen before that last update\<close>
+  shows "\<nexists> caller' token' amount' proof'. CLAIM bridgeAddress caller' ID token' amount' proof' \<in> set stepsInit"
+proof (rule ccontr)
+  assume "\<not> ?thesis"
+  then obtain caller' token' amount' proof' where 
+    *: "CLAIM bridgeAddress caller' ID token' amount' proof' \<in> set stepsInit"
+    by auto
+  then have "getClaim (the (bridgeState contractsLastUpdate' bridgeAddress)) ID = True"
+    using claimStepSetsClaim reachableFromInitLastUpdate'
+    by blast
+
+  moreover
+
+  have "verifyClaimProof () bridgeAddress ID stateRoot proof = True"
+    by (metis properSetupBD properSetup_def bridgeDeadContractsBD callCancelDepositWhileDeadVerifyClaimProof cancel deadStateContractsBD lastValidState_def snd_conv)
+  then have "getClaim (the (bridgeState contractsLastUpdate' bridgeAddress)) ID = False"
+    by (metis generateStateRootLastUpdate' option.collapse properSetupLastUpdate' properSetup_def verifyClaimProofE)
+
+  ultimately
+
+  show False
+    by simp
+qed
+
+(* FIXME: could this special case be somehow avoided? *)
+theorem cancelDepositWhileDeadNoClaimDeathStep:
+  assumes "stepDeath = CANCEL tokenDepositAddress caller ID token amount proof"
+  shows "\<nexists> caller' token' amount' proof'. CLAIM bridgeAddress caller' ID token' amount' proof' \<in> set stepsInit"
+proof (rule ccontr)
+  assume "\<not> ?thesis"
+  then obtain caller' token' amount' proof' where 
+    *: "CLAIM bridgeAddress caller' ID token' amount' proof' \<in> set stepsInit"
+    by auto
+  then have "getClaim (the (bridgeState contractsLastUpdate' bridgeAddress)) ID = True"
+    using claimStepSetsClaim reachableFromInitLastUpdate'
+    by blast
+
+  moreover
+
+  thm callCancelDepositWhileDead_def
+  obtain block where cancel: "callCancelDepositWhileDead contractsDead' tokenDepositAddress (message caller 0) block ID token amount proof = (Success, contractsDead)"
+    using deathStep assms
+    by (smt (verit, ccfv_threshold) executeStep.simps(4) list.discI list.inject reachableFrom.cases)
+  have "verifyClaimProof () bridgeAddress ID stateRoot proof = True"
+    using callCancelDepositWhileDeadVerifyClaimProof[OF cancel]
+    by (smt (verit, best) callLastState callLastStateI getLastStateBDead' lastValidState_def notBridgeDead' prod.exhaust_sel properSetupDead' properSetup_def)
+  then have "getClaim (the (bridgeState contractsLastUpdate' bridgeAddress)) ID = False"
+    by (metis generateStateRootLastUpdate' option.collapse properSetupLastUpdate' properSetup_def verifyClaimProofE)
+
+  ultimately
+
+  show False
+    by simp
+qed
+
+text \<open>If withdrawal succeeds, then the bridge is dead and 
+      the user had the exact amount of tokens in the state in which the bridge died\<close>
+theorem withdrawSufficientBalance:
+  \<comment> \<open>Token deposit can accept token\<close>
+  assumes "properToken contractsInit tokenDepositAddress bridgeAddress token"
+  \<comment> \<open>Withdraw succeded\<close>
+  assumes withdraw:
+    "callWithdrawWhileDead contractsBD tokenDepositAddress msg block token amount proof = (Success, contractsW)"
+  \<comment> \<open>Caller had sufficient balance\<close>
+  shows "callBalanceOf contractsLastUpdate' token (sender msg) = (Success, amount)"
+proof-
+  have "verifyBalanceProof () token (sender msg) amount stateRoot proof"
+    using callWithdrawWhileDeadVerifyBalanceProof[OF withdraw]
+    by (metis bridgeDeadContractsBD deadStateContractsBD lastValidState_def snd_conv)
+  then have "balanceOf (the (ERC20state contractsLastUpdate' token)) (sender msg) = amount"
+    using assms
+    using verifyBalanceProofE[of contractsLastUpdate' stateRoot]
+    by auto
+  then show ?thesis
+    using assms
+    unfolding callBalanceOf_def
+    by (auto split: option.splits)
+qed
+
+
+(* FIXME: could this special case be somehow avoided? *)
+theorem withdrawSufficientBalanceDeathStep:
+  \<comment> \<open>Token deposit can accept token\<close>
+  assumes "properToken contractsInit tokenDepositAddress bridgeAddress token"
+  \<comment> \<open>Withdraw succeded\<close>
+  assumes "stepDeath = WITHDRAW tokenDepositAddress caller token amount proof"
+  \<comment> \<open>Caller had sufficient balance\<close>
+  shows "callBalanceOf contractsLastUpdate' token caller = (Success, amount)"
+proof-
+  obtain block where
+    withdraw: "callWithdrawWhileDead contractsDead' tokenDepositAddress (message caller 0) block token amount proof = 
+    (Success, contractsDead)"
+    using deathStep assms
+    by (smt (verit) executeStep.simps(5) list.discI reachableFrom.simps reachableFromCons')
+  have "verifyBalanceProof () token caller amount stateRoot proof"
+    using callWithdrawWhileDeadVerifyBalanceProof[OF withdraw]
+    by (smt (verit) callLastState callLastStateI getLastStateTDDead' lastValidState_def notBridgeDead' prod.exhaust_sel properSetupDead' properSetup_def senderMessage)
+  then have "balanceOf (the (ERC20state contractsLastUpdate' token)) caller = amount"
+    using assms
+    using verifyBalanceProofE[of contractsLastUpdate' stateRoot]
+    by auto
+  then show ?thesis
+    using assms
+    unfolding callBalanceOf_def
+    by (auto split: option.splits)
+qed
+
+end
+
+context HashProofVerifier
+begin
+
+fun isTokenCancel where
+  "isTokenCancel address token (CANCEL address' caller ID token' amount proof) \<longleftrightarrow> address' = address \<and> token' = token"
+| "isTokenCancel address token _ = False"
+
+definition tokenCancels where
+  "tokenCancels address token steps = 
+   filter (isTokenCancel address token) steps"
+
+definition canceledTokenAmount where
+  "canceledTokenAmount address token steps = 
+   sum_list (map CANCEL_amount (tokenCancels address token steps))"
+
+lemma canceledTokenAmountCancel [simp]:
+  shows "canceledTokenAmount address token (CANCEL address caller ID token amount proof # steps) = 
+         amount + canceledTokenAmount address token steps"
+  unfolding canceledTokenAmount_def tokenCancels_def
+  by auto
+
+lemma canceledAmountConsNonCancel [simp]:
+  assumes "\<nexists> address' caller' ID' token' amount' proof'. step = CANCEL address' caller' ID' token' amount' proof'"
+  shows "canceledTokenAmount address token (step # steps) = canceledTokenAmount address token steps"
+  using assms 
+  unfolding canceledTokenAmount_def tokenCancels_def
+  by (cases step, auto)
+
+lemma canceledTokenAmountConsOther [simp]:
+  assumes "address \<noteq> address' \<or> token \<noteq> token'"
+  shows "canceledTokenAmount address token (CANCEL address' caller' ID' token' amount' proof' # steps) = 
+         canceledTokenAmount address token steps"
+  using assms
+  unfolding canceledTokenAmount_def tokenCancels_def
+  by auto
+
+definition nonClaimedBeforeDeathTokenDeposits where
+  "nonClaimedBeforeDeathTokenDeposits tokenDepositAddress bridgeAddress token stepsBefore steps =
+     filter (\<lambda> step. \<not> isClaimedID bridgeAddress token (DEPOSIT_id step) stepsBefore) 
+            (tokenDeposits tokenDepositAddress token steps)"
+
+definition isCanceledID where
+  "isCanceledID tokenDepositAddress token ID steps \<longleftrightarrow> 
+   (\<exists> caller amount proof. CANCEL tokenDepositAddress caller ID token amount proof \<in> set steps)"
+
+definition nonCanceledNonClaimedBeforeDeathTokenDeposits where
+  "nonCanceledNonClaimedBeforeDeathTokenDeposits tokenDepositAddress bridgeAddress token stepsBefore steps =
+     filter (\<lambda> step. \<not> isClaimedID bridgeAddress token (DEPOSIT_id step) stepsBefore \<and>
+                     \<not> isCanceledID tokenDepositAddress token (DEPOSIT_id step) steps)
+            (tokenDeposits tokenDepositAddress token steps)"
+
+definition tokenWithdrawals where
+  "tokenWithdrawals address token steps = filter (\<lambda> step. case step of WITHDRAW address' caller token' amount proof \<Rightarrow> address = address' \<and> token = token' | _ \<Rightarrow> False) steps"
+
+definition tokenWithdrawnAmount where
+  "tokenWithdrawnAmount address token steps = 
+   sum_list (map WITHDRAW_amount (tokenWithdrawals address token steps))"
+
+lemma tokenWithdrawnAmoutConsNonWithdraw [simp]:
+  assumes "\<nexists> address' caller' token' amount' proof'. step = WITHDRAW address' caller' token' amount' proof'"
+  shows "tokenWithdrawnAmount address token (step # steps) = tokenWithdrawnAmount address token steps"
+  using assms 
+  unfolding tokenWithdrawnAmount_def tokenWithdrawals_def
+  by (cases step, auto)
+
+end
+
+
+(**************************************************************************************************)
+section \<open>Liveness\<close>
+(**************************************************************************************************)
+
+context LastUpdate
+begin
+
+(*
+               deposit                [steps]                      update                        [steps']                   claim?        
+   contracts      \<rightarrow>    contractsD       \<rightarrow>*   contractsLastUpdate'     \<rightarrow>   contractsLastUpdate   \<rightarrow>*      contractsU'      \<rightarrow>    contractsC?
+  properSetup                                     \<not> bridgeDead                                   noUpdates   \<not> getClaim ID
+  properToken
+*)
+
+text \<open>After a successful deposit and a state update, 
+      if a bridge is still alive a claim can be made \<close>
+theorem claimPossibleAfterDepositAndUpdate:
+  \<comment> \<open>contracts are setup properly in the initial state, for the given token\<close>
+  assumes "properSetup contracts tokenDepositAddress bridgeAddress"
+  assumes "properToken contracts tokenDepositAddress bridgeAddress token"
+
+  \<comment> \<open>A deposit is successfully made\<close>
+  assumes "callDeposit contracts tokenDepositAddress block msg ID token amount = (Success, contractsD)"
+  \<comment> \<open>after a deposit a new state is reached\<close>
+  assumes "reachableFrom contractsD contractsLastUpdate' steps"
+  \<comment> \<open>the bridge is not dead in the reached state\<close>
+  assumes "\<not> bridgeDead  contractsLastUpdate' tokenDepositAddress"
+
+  \<comment> \<open>there was no previous claim\<close>
+  assumes "getClaim (the (bridgeState contractsLU bridgeAddress)) ID = False"
+
+  \<comment> \<open>The same person who made the deposit can make the claim\<close>
+  assumes "sender msg' = sender msg"
+
+  \<comment> \<open>A claim can be made with the state root and the proof obtained from the state that
+      was used for the last update\<close>
+  shows "let proof = generateDepositProof contractsLastUpdate' ID
+          in \<exists> contractsC. callClaim contractsLU bridgeAddress msg' ID token amount proof = (Success, contractsC)"
+proof-
+  define "proof" where "proof = generateDepositProof contractsLastUpdate' ID"
+  define stateBridge where "stateBridge = the (bridgeState contractsLU bridgeAddress)"
+
+  have *: "verifyDepositProof () tokenDepositAddress ID (hash3 (sender msg) token amount) stateRoot proof = True"
+    unfolding proof_def
+  proof (rule verifyDepositProofI)
+    show "getDeposit (the (tokenDepositState contractsLastUpdate' tokenDepositAddress)) ID = hash3 (sender msg) token amount"
+    proof (rule reachableFromGetDepositBridgeNotDead)
+      show "reachableFrom contractsD contractsLastUpdate' steps" 
+        by fact
+    next
+      show "hash3 (sender msg) token amount \<noteq> 0"
+        using hash3_nonzero
+        by simp
+    next
+      show "getDeposit (the (tokenDepositState contractsD tokenDepositAddress)) ID = hash3 (sender msg) token amount"
+        using callDepositWritesHash assms
+        by blast
+    next
+      show "\<not> bridgeDead contractsLastUpdate' tokenDepositAddress"
+        using assms
+        by simp
+    qed
+  qed simp_all
+  then have "verifyDepositProof () (BridgeState.deposit stateBridge) ID (hash3 (sender msg') token amount)
+     (getLastStateB contractsLU bridgeAddress) proof"
+    using \<open>sender msg' = sender msg\<close> depositLU getLastStateBLU stateBridge_def
+    by argo
+
+  then have "fst (callClaim contractsLU bridgeAddress msg' ID token amount proof) = Success"
+    by (smt (verit, ccfv_threshold) HashProofVerifier.callClaimI HashProofVerifier_axioms assms(2) assms(3) assms(4) assms(6) callDepositProperToken option.collapse properSetupLU properSetup_def properTokenReachable properToken_def reachableFromLastUpdate'LU stateBridge_def)
+  then show ?thesis 
+    unfolding Let_def proof_def
+    by (metis eq_fst_iff)
+qed
+
+end
+
+
+context BridgeDead
+begin
+
+text \<open>If the user had some amount of tokens in the state in which the bridge died, 
+      he can withdraw that amount\<close>
+theorem sufficientBalanceCanWithdraw:
+  \<comment> \<open>Token deposit can accept token\<close>
+  assumes "properToken contractsInit tokenDepositAddress bridgeAddress token"
+  \<comment> \<open>Caller had sufficient balance\<close>
+  assumes "callBalanceOf contractsLastUpdate' token (sender msg) = (Success, amount)"
+  \<comment> \<open>Caller has not yet withdrawn his balance\<close>
+  assumes notWithdrawn: 
+    "getTokenWithdrawn (the (tokenDepositState contractsBD tokenDepositAddress)) (hash2 (sender msg) token) = False"
+  \<comment> \<open>Sender is not the bridge itself\<close>
+  assumes "tokenDepositAddress \<noteq> sender msg"
+  \<comment> \<open>Withdraw succedes\<close>
+  shows "fst (callWithdrawWhileDead contractsBD tokenDepositAddress msg block token amount 
+                                    (generateBalanceProof contractsLastUpdate' token (sender msg) amount)) = Success"
+proof-
+  define stateTokenDeposit where "stateTokenDeposit = the (tokenDepositState contractsBD tokenDepositAddress)"
+  define stateTokenDeposit' where "stateTokenDeposit' = snd (snd (getDeadStatus contractsBD stateTokenDeposit block))"
+  define Proof where "Proof =  generateBalanceProof contractsLastUpdate' token (sender msg) amount"
+
+  have "verifyBalanceProof () token (sender msg) amount stateRoot Proof = True"
+    using verifyBalanceProofI \<open>callBalanceOf contractsLastUpdate' token (sender msg) = (Success, amount)\<close>
+    unfolding Proof_def
+    by (metis callBalanceOf callBalanceOfERC20state generateStateRootLastUpdate' option.collapse)
+
+  moreover
+
+  have "proofVerifierState contractsBD (TokenDepositState.proofVerifier stateTokenDeposit) \<noteq> None"
+     by (metis properSetupBD properSetup_def stateTokenDeposit_def)
+
+  moreover
+
+  have "deadState stateTokenDeposit' = stateRoot"
+    by (metis bridgeDeadContractsBD deadStateContractsBD getDeadStatusInDeadState prod.exhaust_sel stateTokenDeposit'_def stateTokenDeposit_def)
+
+  ultimately
+  
+  have "callVerifyBalanceProof contractsBD (TokenDepositState.proofVerifier stateTokenDeposit) token (sender msg) amount
+        (deadState stateTokenDeposit') Proof = Success"
+    unfolding callVerifyBalanceProof_def
+    by (auto split: option.splits)
+
+  moreover
+
+  have "getDeadStatus contractsBD stateTokenDeposit block = (Success, True, stateTokenDeposit')"
+    by (metis deadStateContractsBD getDeadStatus_def split_pairs stateRootNonZero stateTokenDeposit'_def stateTokenDeposit_def)
+
+  moreover
+
+  have "fst (callSafeTransferFrom contractsBD token tokenDepositAddress (sender msg) amount) = Success"
+  proof (rule callSafeTransferFromI)
+    show "ERC20state contractsBD token = Some (the (ERC20state contractsBD token))"
+      using \<open>properToken contractsInit tokenDepositAddress bridgeAddress token\<close>
+      by simp
+  next
+    show "tokenDepositAddress \<noteq> sender msg"
+      by fact
+  next
+    show "amount \<le> balanceOf (the (ERC20state contractsBD token)) tokenDepositAddress"
+      sorry
+  qed
+
+  ultimately
+
+  show ?thesis
+    using notWithdrawn
+    unfolding stateTokenDeposit'_def stateTokenDeposit_def Proof_def
+    unfolding callWithdrawWhileDead_def withdrawWhileDead_def
+    by (auto simp add: Let_def split: option.splits prod.splits if_split_asm)
+qed
+
+end
+
+
+(*
+
+(* ------------------------------------------------------------------------------------ *)
+
+
+context ProofVerifier
+begin
+
+(* ----------------------------------------------------------------------------------------- *)
+
+
+(* ------------------------------------------------------------------- *)
+
+
+lemma nonClaimedBeforeDeathTokenDepositsDeposit:
+  assumes "reachableFrom contractsInit contracts (DEPOSIT tokenDepositAddress caller ID token amount # steps @ stepsBefore)"
+  shows "nonClaimedBeforeDeathTokenDeposits tokenDepositAddress bridgeAddress token stepsBefore (DEPOSIT tokenDepositAddress caller ID token amount # steps @ stepsBefore) =
+         (DEPOSIT tokenDepositAddress caller ID token amount) # nonClaimedBeforeDeathTokenDeposits tokenDepositAddress bridgeAddress token stepsBefore (steps @ stepsBefore)"
+  using assms
+  unfolding nonClaimedBeforeDeathTokenDeposits_def
+  apply (auto simp add: tokenDeposits_def)
+  sorry
+
+lemma nonCanceledNonClaimedTokenDepositsBeforeDeathDeposit:
+  assumes "reachableFrom contractsInit contracts (DEPOSIT tokenDepositAddress caller ID token amount # steps @ stepsBefore)"
+  shows "nonCanceledNonClaimedBeforeDeathTokenDeposits tokenDepositAddress bridgeAddress token stepsBefore (DEPOSIT tokenDepositAddress caller ID token amount # steps @ stepsBefore) =
+         (DEPOSIT tokenDepositAddress caller ID token amount) # nonCanceledNonClaimedBeforeDeathTokenDeposits tokenDepositAddress bridgeAddress token stepsBefore (steps @ stepsBefore)"
+  using assms
+  unfolding nonCanceledNonClaimedBeforeDeathTokenDeposits_def
+  apply (auto simp add: tokenDeposits_def)
+  sorry
+
+
+lemma nonCanceledNonClaimedBeforeDeathTokenDepositsCancel:
+  assumes "reachableFrom contractsInit contracts stepsBefore"
+  \<comment> \<open>The last update that happened when the bridge was still alive\<close>
+  assumes update:
+          "let stateOracleAddress = BridgeState.stateOracle (the (bridgeState contractsInit bridgeAddress))
+            in callUpdate contracts stateOracleAddress block blockNum stateRoot = (Success, contracts')"
+  assumes "stateRoot \<noteq> 0" (* NOTE: additional assumption *)
+  assumes "\<not> (bridgeDead contracts tokenDepositAddress)"
+  \<comment> \<open>There were no updates since then\<close>
+  assumes "reachableFrom contracts' contracts'' steps'"
+  assumes noUpdate: "let stateOracleAddress = BridgeState.stateOracle (the (bridgeState contractsInit bridgeAddress))
+            in \<nexists> stateRoot'. UPDATE stateOracleAddress stateRoot' \<in> set steps'"
+  \<comment> \<open>Bridge was dead\<close>
+  assumes "\<not> (bridgeDead contracts'' tokenDepositAddress)"
+  assumes "stepsF = [CANCEL tokenDepositAddress caller ID token amount proof] @ steps'' @ steps' @ [UPDATE tokenDepositAddress stateRoot] @ stepsBefore"
+  shows "\<exists> steps1 steps2.
+           nonCanceledNonClaimedBeforeDeathTokenDeposits tokenDepositAddress bridgeAddress token stepsBefore (steps @ stepsBefore) = 
+           steps1 @ [DEPOSIT tokenDepositAddress caller ID token amount] @ steps2 \<and>
+           nonCanceledNonClaimedBeforeDeathTokenDeposits tokenDepositAddress bridgeAddress token stepsBefore (CANCEL tokenDepositAddress caller ID token amount proof # steps @ stepsBefore) = 
+           steps1 @ steps2"
+proof-
+  define CANCEL_step where "CANCEL_step = CANCEL tokenDepositAddress caller ID token amount proof"
+  define DEPOSIT_step where "DEPOSIT_step = DEPOSIT tokenDepositAddress (sender (message caller 0)) ID token amount"
+
+  obtain contracts' block where 
+     "reachableFrom contractsInit contracts' (steps @ stepsBefore)" 
+     "callCancelDepositWhileDead contracts' tokenDepositAddress (message caller 0) block ID token amount proof = (Success, contracts)"
+    using reachableFromCons'[OF assms(1)]
+    by auto
+
+  then obtain contractsLast where
+    "reachableFrom contractsInit contractsLast stepsBefore"
+    "reachableFrom contractsLast contracts' steps"
+    using reachableFromAppend by blast
+
+  have "DEPOSIT_step \<in> set (steps @ stepsBefore)"
+    unfolding DEPOSIT_step_def
+  proof (rule cancelDepositOnlyAfterDeposit)
+    show "callCancelDepositWhileDead contracts' tokenDepositAddress (message caller 0) block ID token amount proof = (Success, contracts)"
+      by fact
+  next
+    show "reachableFrom contractsInit contracts' (steps @ stepsBefore)"
+      by fact
+  next
+    show "properSetup contractsInit tokenDepositAddress bridgeAddress"
+      by fact
+  next
+    show "getDeposit (the (tokenDepositState contractsInit tokenDepositAddress)) ID = 0"
+      sorry
+  next
+    show "hash3 (sender (message caller 0)) token amount \<noteq> 0"
+      sorry
+  next
+    show "hash3_inj"
+      sorry
+  qed
+  then obtain steps1 steps2 where steps: "steps @ stepsBefore = steps1 @ [DEPOSIT_step] @ steps2"
+    by (metis append_Cons append_self_conv2 split_list)
+  then have "DEPOSIT_step \<in> set (tokenDeposits tokenDepositAddress token (steps @ stepsBefore))"
+    unfolding tokenDeposits_def DEPOSIT_step_def
+    by auto
+
+  moreover
+
+  have "\<nexists> caller' token' amount' proof'. CLAIM bridgeAddress caller' ID token' amount' proof' \<in> set stepsBefore"
+  proof (rule cancelDepositNoClaim)
+    show "callCancelDepositWhileDead contracts' tokenDepositAddress (message caller 0) block ID token amount proof = (Success, contracts)"
+      by fact
+  next
+    show "reachableFrom contractsInit contractsLast stepsBefore"
+      by fact
+  next
+    show "properSetup contractsInit tokenDepositAddress bridgeAddress"
+      by fact
+  next
+  qed
+
+  moreover
+  have "\<nexists> caller' amount' proof'. 
+          CANCEL tokenDepositAddress caller' ID token amount' proof' \<in> set (steps @ stepsBefore)"
+    sorry
+
+  ultimately
+
+  have "DEPOSIT_step \<in> set (nonCanceledNonClaimedBeforeDeathTokenDeposits tokenDepositAddress bridgeAddress token stepsBefore (steps @ stepsBefore))"
+    unfolding nonCanceledNonClaimedBeforeDeathTokenDeposits_def DEPOSIT_step_def isClaimedID_def isCanceledID_def
+    by auto
+
+  have *: "\<forall> step \<in> set (steps1 @ steps2). (\<forall> caller' amount' ID'. step = DEPOSIT tokenDepositAddress caller' ID' token amount' \<longrightarrow> ID' \<noteq> ID)"
+  proof safe
+    fix caller' amount' proof' 
+    assume "DEPOSIT tokenDepositAddress caller' ID token amount' \<in> set (steps1 @ steps2)"
+    moreover
+    have "\<nexists>token' caller' amount'.
+         DEPOSIT tokenDepositAddress caller' ID token' amount' \<in> set (steps1 @ steps2)"
+    proof (rule DEPOSITNoDouble')
+      show "steps @ stepsBefore = steps1 @ [DEPOSIT tokenDepositAddress caller ID token amount] @ steps2"
+        using steps
+        unfolding DEPOSIT_step_def
+        by simp
+    next
+      show "depositHashesNonZero (steps @ stepsBefore)"
+        sorry
+    next
+      show "reachableFrom contractsInit contracts' (steps @ stepsBefore)"
+        by fact
+    qed
+    ultimately
+    show False
+      by simp
+  qed
+  then have "DEPOSIT_step \<notin> set (steps1 @ steps2)"
+    unfolding DEPOSIT_step_def
+    by auto
+
+  show ?thesis
+    using cancelDepositNoClaim
+    sorry
+qed
+
+lemma nonClaimedTokenDepositsBeforeDeathOther [simp]:
+  assumes "\<nexists> caller' ID' amount'. step = DEPOSIT tokenDepositAddress caller' ID' token amount'"
+  shows "nonClaimedTokenDepositsBeforeDeath tokenDepositAddress bridgeAddress token stepsBefore (step # steps) =
+         nonClaimedTokenDepositsBeforeDeath tokenDepositAddress bridgeAddress token stepsBefore steps"
+  using assms
+  unfolding nonClaimedTokenDepositsBeforeDeath_def tokenDeposits_def
+  by (auto split: Step.splits)
+
+lemma nonCanceledNonClaimedTokenDepositsBeforeDeathOther [simp]:
+  assumes "\<nexists> caller' ID' amount'. step = DEPOSIT tokenDepositAddress caller' ID' token amount'"
+  assumes "\<nexists> caller' ID' amount' proof'. step = CANCEL tokenDepositAddress caller' ID' token amount' proof'"
+  shows "nonCanceledNonClaimedTokenDepositsBeforeDeath tokenDepositAddress bridgeAddress token stepsBefore (step # steps) =
+         nonCanceledNonClaimedTokenDepositsBeforeDeath tokenDepositAddress bridgeAddress token stepsBefore steps"
+  using assms
+  unfolding nonCanceledNonClaimedTokenDepositsBeforeDeath_def tokenDeposits_def
+  by (auto split: Step.splits)
+
+definition nonCanceledNonClaimedTokenDepositsBeforeDeathAmount where
+  "nonCanceledNonClaimedTokenDepositsBeforeDeathAmount tokenDepositAddress bridgeAddress token stepsBefore steps =
+    sum_list (map DEPOSIT_amount (nonCanceledNonClaimedTokenDepositsBeforeDeath tokenDepositAddress bridgeAddress token stepsBefore steps))"
+
+definition nonClaimedTokenDepositsBeforeDeathAmount where
+  "nonClaimedTokenDepositsBeforeDeathAmount tokenDepositAddress bridgeAddress token stepsBefore steps =
+    sum_list (map DEPOSIT_amount (nonClaimedTokenDepositsBeforeDeath tokenDepositAddress bridgeAddress token stepsBefore steps))"
+
+lemma nonClaimedTokenDepositsBeforeDeathAmountDeposit [simp]:
+  assumes "reachableFrom contractsInit contracts (DEPOSIT tokenDepositAddress caller ID token amount # steps @ stepsBefore)"
+  shows "nonClaimedTokenDepositsBeforeDeathAmount tokenDepositAddress bridgeAddress token stepsBefore (DEPOSIT tokenDepositAddress caller ID token amount # steps @ stepsBefore) =
+         amount + nonClaimedTokenDepositsBeforeDeathAmount tokenDepositAddress bridgeAddress token stepsBefore (steps @ stepsBefore)"
+  using assms nonClaimedTokenDepositsBeforeDeathAmount_def nonClaimedTokenDepositsBeforeDeathDeposit by auto
+
+lemma nonCanceledNonClaimedTokenDepositsBeforeDeathAmountDeposit [simp]:
+  assumes "reachableFrom contractsInit contracts (DEPOSIT tokenDepositAddress caller ID token amount # steps @ stepsBefore)"
+  shows "nonCanceledNonClaimedTokenDepositsBeforeDeathAmount tokenDepositAddress bridgeAddress token stepsBefore (DEPOSIT tokenDepositAddress caller ID token amount # steps @ stepsBefore) =
+         amount + nonCanceledNonClaimedTokenDepositsBeforeDeathAmount tokenDepositAddress bridgeAddress token stepsBefore (steps @ stepsBefore)"
+  using assms nonCanceledNonClaimedTokenDepositsBeforeDeathAmount_def nonCanceledNonClaimedTokenDepositsBeforeDeathDeposit by auto
+
+lemma nonCanceledNonClaimedTokenDepositsBeforeDeathAmountOther [simp]:
+  assumes "\<nexists> caller' ID' amount'. step = DEPOSIT tokenDepositAddress caller' ID' token amount'"
+  assumes "\<nexists> caller' ID' amount' proof'. step = CANCEL tokenDepositAddress caller' ID' token amount' proof'"
+  shows "nonCanceledNonClaimedTokenDepositsBeforeDeathAmount tokenDepositAddress bridgeAddress token stepsBefore (step # steps) =
+         nonCanceledNonClaimedTokenDepositsBeforeDeathAmount tokenDepositAddress bridgeAddress token stepsBefore steps"
+  by (simp add: assms nonCanceledNonClaimedTokenDepositsBeforeDeathAmount_def)
+
+lemma nonClaimedTokenDepositsBeforeDeathAmountOther [simp]:
+  assumes "\<nexists> caller' ID' amount'. step = DEPOSIT tokenDepositAddress caller' ID' token amount'"
+  shows "nonClaimedTokenDepositsBeforeDeathAmount tokenDepositAddress bridgeAddress token stepsBefore (step # steps) =
+         nonClaimedTokenDepositsBeforeDeathAmount tokenDepositAddress bridgeAddress token stepsBefore steps"
+  by (simp add: assms nonClaimedTokenDepositsBeforeDeathAmount_def)
+
+lemma nonCanceledNonClaimedTokenDepositsBeforeDeathAmountCancel:
+  assumes "reachableFrom contractsInit contracts (CANCEL tokenDepositAddress caller ID token amount proof # steps @ stepsBefore)"
+  shows "nonCanceledNonClaimedTokenDepositsBeforeDeathAmount tokenDepositAddress bridgeAddress token stepsBefore (CANCEL tokenDepositAddress caller ID token amount proof # steps @ stepsBefore) =
+         nonCanceledNonClaimedTokenDepositsBeforeDeathAmount tokenDepositAddress bridgeAddress token stepsBefore (steps @ stepsBefore) - amount"
+        "amount \<le> nonCanceledNonClaimedTokenDepositsBeforeDeathAmount tokenDepositAddress bridgeAddress token stepsBefore (steps @ stepsBefore)"
+  using nonCanceledNonClaimedTokenDepositsBeforeDeathCancel[OF assms, of bridgeAddress]
+  unfolding nonCanceledNonClaimedTokenDepositsBeforeDeathAmount_def
+  by auto
+
+
+lemma noCancelBeforeBridgeDead:
+  assumes "reachableFrom contractsInit contracts steps"
+          "\<not> (bridgeDead contracts tokenDepositAddress)"
+  shows "\<nexists> step. step \<in> set steps \<and> (\<exists> caller ID token amount proof. step = CANCEL tokenDepositAddress caller ID token amount proof)"
+  using assms
+proof (induction contractsInit contracts steps rule: reachableFrom.induct)
+  case (reachableFrom_base contracts)
+  then show ?case
+    by simp
+next
+  case (reachableFrom_step steps contracts' contractsInit contracts blockNum block step)
+  have notDead: "\<not> bridgeDead contracts tokenDepositAddress"
+    by (meson ProofVerifier.reachableFromDeadState ProofVerifier.reachableFrom_step ProofVerifier_axioms reachableFrom_base reachableFrom_step.hyps(2) reachableFrom_step.prems)
+  then show ?case
+    using reachableFrom_step callCancelDepositWhileDeadBridgeDead
+    by (metis executeStep.simps(4) set_ConsD)
+qed
+
+lemma canceledTokenAmountBridgeNotDead:
+  assumes "reachableFrom contractsInit contracts steps"
+          "\<not> (bridgeDead contracts tokenDepositAddress)"
+    shows "canceledTokenAmount tokenDepositAddress token steps = 0"
+  using assms noCancelBeforeBridgeDead[OF assms]
+  unfolding canceledTokenAmount_def tokenCancels_def
+  by (auto split: Step.splits)
+
+
+lemma nonCanceledNonClaimedBridgeNotDead:
+  assumes "reachableFrom contractsInit contracts steps"
+          "\<not> (bridgeDead contracts tokenDepositAddress)"
+    shows "nonCanceledNonClaimedTokenDepositsBeforeDeathAmount tokenDepositAddress bridgeAddress token stepsBefore steps =
+           nonClaimedTokenDepositsBeforeDeathAmount tokenDepositAddress bridgeAddress token stepsBefore steps"
+  using assms noCancelBeforeBridgeDead[OF assms]
+  unfolding nonCanceledNonClaimedTokenDepositsBeforeDeathAmount_def nonClaimedTokenDepositsBeforeDeathAmount_def
+  unfolding nonCanceledNonClaimedTokenDepositsBeforeDeath_def nonClaimedTokenDepositsBeforeDeath_def
+  by metis
+
+lemma
+  assumes "reachableFrom contracts'' contractsF steps''"
+  assumes "properSetup contractsInit tokenDepositAddress bridgeAddress"
+  assumes "properToken contractsInit tokenDepositAddress bridgeAddress token"
+
+  assumes "reachableFrom contractsInit contracts stepsBefore"
+  \<comment> \<open>The last update that happened when the bridge was still alive\<close>
+  assumes update:
+          "let stateOracleAddress = BridgeState.stateOracle (the (bridgeState contractsInit bridgeAddress))
+            in callUpdate contracts stateOracleAddress block blockNum stateRoot = (Success, contracts')"
+  assumes "stateRoot \<noteq> 0" (* NOTE: additional assumption *)
+  assumes "\<not> (bridgeDead contracts tokenDepositAddress)"
+  \<comment> \<open>There were no updates since then\<close>
+  assumes "reachableFrom contracts' contracts'' steps'"
+  assumes noUpdate: "let stateOracleAddress = BridgeState.stateOracle (the (bridgeState contractsInit bridgeAddress))
+            in \<nexists> stateRoot'. UPDATE stateOracleAddress stateRoot' \<in> set steps'"
+  \<comment> \<open>Bridge was dead\<close>
+  assumes "\<not> (bridgeDead contracts'' tokenDepositAddress)"
+  assumes "stepsF = steps'' @ steps' @ [UPDATE tokenDepositAddress stateRoot] @ stepsBefore"
+  shows
+  "nonCanceledNonClaimedTokenDepositsBeforeDeathAmount tokenDepositAddress bridgeAddress token stepsBefore stepsF + 
+   canceledTokenAmount tokenDepositAddress token stepsF = 
+   nonClaimedTokenDepositsBeforeDeathAmount tokenDepositAddress bridgeAddress token stepsBefore stepsF"
+  using assms
+proof (induction contracts'' contractsF steps'' arbitrary: stepsF rule: reachableFrom.induct )
+  case (reachableFrom_base contractsF)
+  have "reachableFrom contracts contracts' [UPDATE tokenDepositAddress stateRoot]"
+    sorry
+  then have "reachableFrom contractsInit contractsF stepsF"
+    using reachableFrom_base
+    by (smt (verit, ccfv_threshold) append_Nil reachableFromTrans)
+  moreover
+  have "\<not> (bridgeDead contracts tokenDepositAddress)"
+    using reachableFrom_base
+    by simp
+  ultimately
+  show ?case
+    using canceledTokenAmountBridgeNotDead nonCanceledNonClaimedBridgeNotDead reachableFrom_base
+    by simp
+next
+  case (reachableFrom_step steps contractsF contracts'' contractsF' blockNum block step)
+
+  have "reachableFrom contracts contracts' [UPDATE tokenDepositAddress stateRoot]"
+    sorry
+  then have "reachableFrom contractsInit contractsF stepsF"
+    using reachableFrom_step
+    by (meson reachableFrom.reachableFrom_step reachableFromTrans)
+  
+  define stepsF' where "stepsF' = steps @ steps' @ [UPDATE tokenDepositAddress stateRoot] @ stepsBefore"
+  have *: "nonCanceledNonClaimedTokenDepositsBeforeDeathAmount tokenDepositAddress bridgeAddress token stepsBefore stepsF' +
+           canceledTokenAmount tokenDepositAddress token stepsF' =
+           nonClaimedTokenDepositsBeforeDeathAmount tokenDepositAddress bridgeAddress token stepsBefore stepsF'"
+    unfolding stepsF'_def
+    using reachableFrom_step
+    by auto
+  show ?case
+  proof (cases step)
+    case (UPDATE address' stateRoot')
+    then show ?thesis
+      using * reachableFrom_step.prems(10)
+      unfolding stepsF'_def
+      by simp
+  next
+    case (WITHDRAW address' caller' token' amount' proof')
+    then show ?thesis
+      using * reachableFrom_step.prems(10)
+      unfolding stepsF'_def
+      by simp
+  next
+    case (CLAIM address' caller' ID' token' amount' proof')
+    then show ?thesis
+      using * reachableFrom_step.prems(10)
+      unfolding stepsF'_def
+      by simp
+  next
+    case (DEPOSIT address' caller' ID' token' amount')
+    show ?thesis
+    proof (cases "address' = tokenDepositAddress \<and> token' = token")
+      case False
+      then show ?thesis
+        using * DEPOSIT reachableFrom_step.prems(10)
+        unfolding stepsF'_def
+        by simp
+    next
+      case True
+      have "nonClaimedTokenDepositsBeforeDeathAmount tokenDepositAddress bridgeAddress token stepsBefore stepsF =
+            amount' + nonClaimedTokenDepositsBeforeDeathAmount tokenDepositAddress bridgeAddress token stepsBefore stepsF'"
+        using nonClaimedTokenDepositsBeforeDeathAmountDeposit[where steps="steps @ steps' @ [UPDATE tokenDepositAddress stateRoot]"]
+        using \<open>reachableFrom contractsInit contractsF stepsF\<close>
+        unfolding stepsF'_def reachableFrom_step.prems(10)
+        using True * DEPOSIT 
+        by auto
+      moreover
+      have "nonCanceledNonClaimedTokenDepositsBeforeDeathAmount tokenDepositAddress bridgeAddress token stepsBefore stepsF =
+            amount' + nonCanceledNonClaimedTokenDepositsBeforeDeathAmount tokenDepositAddress bridgeAddress token stepsBefore stepsF'"
+        using nonCanceledNonClaimedTokenDepositsBeforeDeathAmountDeposit[where steps="steps @ steps' @ [UPDATE tokenDepositAddress stateRoot]"]
+        using \<open>reachableFrom contractsInit contractsF stepsF\<close>
+        unfolding stepsF'_def reachableFrom_step.prems(10)
+        using True * DEPOSIT 
+        by auto
+      ultimately
+      show ?thesis
+        using True * DEPOSIT reachableFrom_step.prems(10)
+        unfolding stepsF'_def
+        by simp
+    qed
+  next
+    case (CANCEL address' caller' ID' token' amount' proof')
+    show ?thesis
+    proof (cases "address' = tokenDepositAddress \<and> token' = token")
+      case False
+      then show ?thesis
+        using * CANCEL
+        unfolding stepsF'_def reachableFrom_step.prems(10)
+        by auto
+    next
+      case True
+      have "nonCanceledNonClaimedTokenDepositsBeforeDeathAmount tokenDepositAddress bridgeAddress token stepsBefore stepsF = 
+            nonCanceledNonClaimedTokenDepositsBeforeDeathAmount tokenDepositAddress bridgeAddress token stepsBefore stepsF' - 
+            amount'"
+           "amount' \<le> nonCanceledNonClaimedTokenDepositsBeforeDeathAmount tokenDepositAddress bridgeAddress token stepsBefore stepsF'"
+        using \<open>reachableFrom contractsInit contractsF stepsF\<close> nonCanceledNonClaimedTokenDepositsBeforeDeathAmountCancel
+        by (smt (verit, best) CANCEL True append.assoc append_Cons reachableFrom_step.prems(10) stepsF'_def)+
+      then show ?thesis
+        using * True CANCEL
+        unfolding stepsF'_def reachableFrom_step.prems(10)
+        by simp
+    qed
+  qed
+qed
+
+
+
+
+end
+
+*)
 end
